src/prop/PFConsistentStrong2.v
@@ -1,0 +1,2684 @@
+Require Import Omega.
+Require Import Bool.
+Require Import RelationClasses.
+
+From sflib Require Import sflib.
+From Paco Require Import paco.
+
+From PromisingLib Require Import Axioms.
+From PromisingLib Require Import Basic.
+From PromisingLib Require Import DataStructure.
+From PromisingLib Require Import DenseOrder.
+From PromisingLib Require Import Language.
+From PromisingLib Require Import Loc.
+
+Require Import Event.
+Require Import Time.
+Require Import View.
+Require Import Cell.
+Require Import Memory.
+Require Import TView.
+Require Import Local.
+Require Import Thread.
+Require Import Pred.
+Require Import Trace.
+
+Require Import MemoryMerge.
+Require Import PromiseConsistent.
+Require Import PFConsistent.
+Require Import ReorderCancel.
+Require Import MemoryProps.
+Require Import OrderedTimes.
+
+Require Import Mapping.
+Require Import CapFlex.
+Require Import GoodFuture.
+Require Import Cover.
+
+Set Implicit Arguments.
+
+
+Section TEVENTMAP.
+
+  Inductive tevent_map_weak (f: Loc.t -> Time.t -> Time.t -> Prop)
+  : ThreadEvent.t -> ThreadEvent.t -> Prop :=
+  | tevent_map_weak_promise
+      loc from ffrom to fto msg fmsg kind fkind
+      (FROM: f loc from ffrom)
+      (TO: f loc to fto)
+    :
+      tevent_map_weak
+        f
+        (ThreadEvent.promise loc ffrom fto fmsg fkind)
+        (ThreadEvent.promise loc from to msg kind)
+  | tevent_map_weak_read
+      loc to fto val released freleased ordr
+      (TO: f loc to fto)
+    :
+      tevent_map_weak
+        f
+        (ThreadEvent.read loc fto val freleased ordr)
+        (ThreadEvent.read loc to val released ordr)
+  | tevent_map_weak_write
+      loc from ffrom to fto val released freleased ordw
+      (FROM: f loc from ffrom)
+      (TO: f loc to fto)
+    :
+      tevent_map_weak
+        f
+        (ThreadEvent.write loc ffrom fto val freleased ordw)
+        (ThreadEvent.write loc from to val released ordw)
+  | tevent_map_weak_update
+      loc from ffrom to fto valr valw releasedr freleasedr
+      releasedw freleasedw ordr ordw
+      (FROM: f loc from ffrom)
+      (TO: f loc to fto)
+    :
+      tevent_map_weak
+        f
+        (ThreadEvent.update loc ffrom fto valr valw freleasedr freleasedw ordr ordw)
+        (ThreadEvent.update loc from to valr valw releasedr releasedw ordr ordw)
+  | tevent_map_weak_fence
+      or ow
+    :
+      tevent_map_weak
+        f
+        (ThreadEvent.fence or ow)
+        (ThreadEvent.fence or ow)
+  | tevent_map_weak_syscall
+      e
+    :
+      tevent_map_weak
+        f
+        (ThreadEvent.syscall e)
+        (ThreadEvent.syscall e)
+  | tevent_map_weak_silent
+    :
+      tevent_map_weak
+        f
+        (ThreadEvent.silent)
+        (ThreadEvent.silent)
+  | tevent_map_weak_failure
+    :
+      tevent_map_weak
+        f
+        (ThreadEvent.failure)
+        (ThreadEvent.failure)
+  .
+  Hint Constructors tevent_map_weak.
+
+  Lemma tevent_map_tevent_map_weak f e fe
+        (EVENT: tevent_map f e fe)
+    :
+      tevent_map_weak f e fe.
+  Proof.
+    inv EVENT; eauto.
+  Qed.
+
+  Lemma tevent_map_weak_compose (f0 f1 f2: Loc.t -> Time.t -> Time.t -> Prop) e0 e1 e2
+        (EVENT0: tevent_map_weak f0 e1 e0)
+        (EVENT1: tevent_map_weak f1 e2 e1)
+        (COMPOSE: forall loc ts0 ts1 ts2 (MAP0: f0 loc ts0 ts1) (MAP1: f1 loc ts1 ts2),
+            f2 loc ts0 ts2)
+    :
+      tevent_map_weak f2 e2 e0.
+  Proof.
+    inv EVENT0; inv EVENT1; econs; eauto.
+  Qed.
+
+  Lemma tevent_map_weak_rev (f0 f1: Loc.t -> Time.t -> Time.t -> Prop) e0 e1
+        (EVENT: tevent_map_weak f0 e1 e0)
+        (REV: forall loc ts0 ts1 (MAP: f0 loc ts0 ts1), f1 loc ts1 ts0)
+    :
+      tevent_map_weak f1 e0 e1.
+  Proof.
+    inv EVENT; econs; eauto.
+  Qed.
+
+End TEVENTMAP.
+
+Section CONCRETEMAX.
+
+  Inductive concrete_promise_max_ts mem prom loc ts: Prop :=
+  | concrete_or_promise_max_ts_intro
+      (EXISTS:
+         (<<CONCRETE: exists from val released,
+             (<<GET: Memory.get loc ts mem = Some (from, Message.concrete val released)>>)>>) \/
+         (<<PROMISE: exists from msg, (<<GET: Memory.get loc ts prom = Some (from, msg)>>)>>))
+      (CONCRETE: forall to from val released
+                        (GET: Memory.get loc to mem = Some (from, Message.concrete val released)),
+          Time.le to ts)
+      (PROMISE: forall to from msg
+                       (GET: Memory.get loc to prom = Some (from, msg)),
+          Time.le to ts)
+  .
+
+  Lemma concrete_promise_max_ts_inj mem prom loc ts0 ts1
+        (MAX0: concrete_promise_max_ts mem prom loc ts0)
+        (MAX1: concrete_promise_max_ts mem prom loc ts1)
+    :
+      ts0 = ts1.
+  Proof.
+    eapply TimeFacts.antisym.
+    { inv MAX0. des.
+      { eapply MAX1 in GET. auto. }
+      { eapply MAX1 in GET. auto. }
+    }
+    { inv MAX1. des.
+      { eapply MAX0 in GET. auto. }
+      { eapply MAX0 in GET. auto. }
+    }
+  Qed.
+
+  Lemma concrete_promise_max_ts_exists mem prom loc
+        (INHABITED: Memory.inhabited mem)
+    :
+      exists ts, (<<MAX: concrete_promise_max_ts mem prom loc ts>>).
+  Proof.
+    exploit Memory.max_concrete_ts_exists; eauto. intros [max MAX].
+    exploit Memory.max_concrete_ts_spec.
+    { eapply MAX. }
+    { eapply INHABITED. } i. des.
+    destruct (classic (exists to from msg, (<<INHABITED: Memory.get loc to prom = Some (from, msg)>>))).
+    { des. eapply Cell.max_ts_spec in INHABITED0. des.
+      exists (Time.join max (Cell.max_ts (prom loc))). econs.
+      { unfold Time.join. des_ifs; eauto. left. eauto. }
+      { i. etrans; [|eapply Time.join_l].
+        eapply Memory.max_concrete_ts_spec in GET1; eauto. des. auto. }
+      { i. etrans; [|eapply Time.join_r].
+        eapply Cell.max_ts_spec in GET1; eauto. des. auto. }
+    }
+    { exists max. econs.
+      { left. eauto. }
+      { i. eapply Memory.max_concrete_ts_spec in GET0; eauto. des. auto. }
+      { i. exfalso. eauto. }
+    }
+  Qed.
+
+  Lemma concrete_promise_max_ts_max_ts mem prom loc ts
+        (MAX: concrete_promise_max_ts mem prom loc ts)
+        (MLE: Memory.le prom mem)
+    :
+      Time.le ts (Memory.max_ts loc mem).
+  Proof.
+    inv MAX. des.
+    { eapply Memory.max_ts_spec; eauto. }
+    { eapply Memory.max_ts_spec; eauto. }
+  Qed.
+
+  Lemma concrete_promise_max_ts_max_concrete_ts mem prom loc ts max
+        (MAX: concrete_promise_max_ts mem prom loc ts)
+        (CONCRETE: Memory.max_concrete_ts mem loc max)
+    :
+      Time.le max ts.
+  Proof.
+    inv CONCRETE. des. eapply MAX in GET; eauto.
+  Qed.
+
+  Definition concrete_promise_max_timemap mem prom tm: Prop :=
+    forall loc, concrete_promise_max_ts mem prom loc (tm loc).
+
+  Lemma concrete_promise_max_timemap_inj mem prom tm0 tm1
+        (MAX0: concrete_promise_max_timemap mem prom tm0)
+        (MAX1: concrete_promise_max_timemap mem prom tm1)
+    :
+      tm0 = tm1.
+  Proof.
+    extensionality loc.
+    eapply concrete_promise_max_ts_inj; eauto.
+  Qed.
+
+  Lemma concrete_promise_max_timemap_exists mem prom
+        (INHABITED: Memory.inhabited mem)
+    :
+      exists tm, (<<MAX: concrete_promise_max_timemap mem prom tm>>).
+  Proof.
+    eapply choice. i. eapply concrete_promise_max_ts_exists; eauto.
+  Qed.
+
+  Lemma map_ident_concrete_promises mem prom tm (f: Loc.t -> Time.t -> Time.t -> Prop)
+        (MAX: concrete_promise_max_timemap mem prom tm)
+        (IDENT: forall loc ts (TS: Time.le ts (tm loc)), f loc ts ts)
+        (MAPLT: mapping_map_lt f)
+        (CLOSED: Memory.closed mem)
+        (MLE: Memory.le prom mem)
+    :
+      promises_map f prom prom.
+  Proof.
+    assert (CONCRETE: map_ident_concrete f mem).
+    { ii. inv CONCRETE. eapply MAX in GET. auto. }
+    econs.
+    { i. exists to, from, msg. splits; auto.
+      { eapply mapping_map_lt_non_collapsable; eauto. }
+      { eapply IDENT. eapply MAX in GET; eauto. }
+      { eapply map_ident_concrete_closed_message; eauto.
+        eapply MLE in GET. eapply CLOSED; eauto. }
+    }
+    { i. exists fto, ffrom, fmsg. splits; auto.
+      { eapply IDENT. eapply MAX in GET; eauto. }
+      { eapply IDENT. transitivity fto.
+        { eapply memory_get_ts_le; eauto. }
+        { eapply MAX in GET; eauto. }
+      }
+    }
+  Qed.
+
+  Lemma memory_ident_map_concrete_max f mem fmem
+        (MEM: memory_map f mem fmem)
+        (IDENT: forall loc to fto (MAP: f loc to fto), to = fto)
+        loc max fmax
+        (CLOSED: Memory.closed mem)
+        (MAX: Memory.max_concrete_ts mem loc max)
+        (FMAX: Memory.max_concrete_ts fmem loc fmax)
+    :
+      Time.le max fmax.
+  Proof.
+    eapply Memory.max_concrete_ts_spec in MAX; eauto.
+    { des. eapply MEM in GET. des; ss. inv MSG. inv MSGLE.
+      eapply Memory.max_concrete_ts_spec in GET; eauto. des.
+      eapply IDENT in TO. subst. auto. }
+    { eapply CLOSED. }
+  Qed.
+
+  Lemma memory_ident_map_concrete_promise_max_timemap
+        f mem_src mem_tgt prom_src prom_tgt tm_src tm_tgt
+        (MAXSRC: concrete_promise_max_timemap mem_src prom_src tm_src)
+        (MAXTGT: concrete_promise_max_timemap mem_tgt prom_tgt tm_tgt)
+        (LOCAL: promises_map f prom_tgt prom_src)
+        (MEM: memory_map f mem_tgt mem_src)
+        (IDENT: forall loc to fto (MAP: f loc to fto), to = fto)
+    :
+      TimeMap.le tm_tgt tm_src.
+  Proof.
+    ii. specialize (MAXTGT loc). inv MAXTGT. des.
+    { eapply MEM in GET. des; ss.
+      eapply IDENT in TO. subst. inv MSG. inv MSGLE.
+      eapply MAXSRC in GET. auto. }
+    { eapply LOCAL in GET. des; ss.
+      eapply IDENT in TO. subst.
+      eapply MAXSRC in GET. auto. }
+  Qed.
+
+End CONCRETEMAX.
+
+
+Definition pf_consistent_strong lang (e0:Thread.t lang): Prop :=
+  forall mem1 sc1
+         (CAP: Memory.cap e0.(Thread.memory) mem1),
+  exists e1,
+    (<<STEPS0: rtc (tau (@pred_step is_cancel lang)) (Thread.mk _ e0.(Thread.state) e0.(Thread.local) sc1 mem1) e1>>) /\
+    (<<NORESERVE: no_reserves e1.(Thread.local).(Local.promises)>>) /\
+    exists e2,
+      (<<STEPS1: rtc (tau (@pred_step ((promise_free /1\ (fun e => ~ is_cancel e)) /1\ no_sc) lang)) e1 e2>>) /\
+      (__guard__((exists st',
+                     (<<LOCAL: Local.failure_step e2.(Thread.local)>>) /\
+                     (<<FAILURE: Language.step lang ProgramEvent.failure (@Thread.state lang e2) st'>>)) \/
+                 (<<PROMISES: e2.(Thread.local).(Local.promises) = Memory.bot>>))).
+
+Lemma pf_consistent_pf_consistent_strong lang (th: Thread.t lang)
+      (WF: Local.wf th.(Thread.local) th.(Thread.memory))
+      (MEM: Memory.closed th.(Thread.memory))
+      (CONSISTENT: pf_consistent th)
+  :
+    pf_consistent_strong th.
+Proof.
+  assert (INHABITED: Memory.inhabited th.(Thread.memory)).
+  { inv MEM. auto. }
+  ii. exploit Memory.max_concrete_timemap_exists; eauto. intros MAX. des.
+  ii. exploit Memory.max_concrete_timemap_exists.
+  { eapply le_inhabited; eauto. eapply Memory.cap_le; eauto. refl. }
+  i. des. exploit CONSISTENT; eauto. i.
+
+  assert (exists e2,
+             (<<STEPS: rtc (tau (Thread.step true))
+                           (Thread.mk _ (Thread.state th) (Thread.local th)
+                                      tm0 mem1) e2 >>) /\
+             (<<NORESERVES: no_reserves e2.(Thread.local).(Local.promises)>>) /\
+             (__guard__ ((exists e3, (<< FAILURE: Thread.step true ThreadEvent.failure e2 e3 >>)) \/
+                         (<<PROMISES: Local.promises (Thread.local e2) = Memory.bot >>)))).
+  { des.
+    - exploit Thread.rtc_tau_step_future.
+      + eapply rtc_implies; [|apply STEPS].
+        i. inv H. econs; eauto. econs; eauto.
+      + ss. eapply Local.cap_wf; eauto.
+      + ss. eapply Memory.max_concrete_timemap_closed; eauto.
+      + ss. eapply Memory.cap_closed; eauto.
+      + i. des.
+        destruct e2. destruct local. inv WF2. ss.
+        exploit reserves_cancelable; eauto. i. des.
+        esplits.
+        * etrans.
+          { eapply STEPS. }
+          { eapply rtc_implies; [|apply STEPS0].
+            i. inv H. inv TSTEP. inv STEP.
+            unfold is_cancel in SAT. des_ifs.
+            inv STEP0; inv STEP.
+            - econs; eauto. econs; eauto. econs; eauto.
+            - inv LOCAL. }
+        * ss.
+        * left. inv FAILURE; inv STEP. inv LOCAL. inv LOCAL0.
+          exists (Thread.mk _ st2 (Local.mk tview proms1) sc2 mem0).
+          ss. econs 2. econs; eauto. econs; eauto. econs; eauto.
+          eapply cancels_promises_decrease in STEPS0; auto. ss.
+          ii. eapply CONSISTENT0; eauto.
+    - unguard. esplits; eauto. rewrite PROMISES. ii.
+      rewrite Memory.bot_get in GET. clarify. }
+
+  clear x. des.
+  eapply pf_step_promise_free_step_rtc in STEPS.
+  eapply pf_steps_cancels_not_cancels in STEPS; cycle 1.
+  { ss. eapply Local.cap_wf; eauto. }
+  { ss. eapply Memory.cap_closed; eauto. }
+  { ss. eapply Memory.max_concrete_timemap_closed; eauto. } des.
+
+  exploit Thread.rtc_tau_step_future.
+  { eapply thread_steps_pred_steps. eapply STEPS1. }
+  { ss. eapply Local.cap_wf; eauto. }
+  { ss. eapply Memory.max_concrete_timemap_closed; eauto. }
+  { ss. eapply Memory.cap_closed; eauto. }
+  i. des. ss.
+
+  destruct th1. exploit no_sc_any_sc_rtc; try apply STEPS1; ss.
+  { i. unfold is_cancel in PR. des_ifs. }
+  i. des. instantiate (1:=sc1) in STEP. clear STEPS1.
+
+  eexists. splits.
+  { eapply STEP. }
+  { ss. ii. clarify.
+    eapply steps_not_cancel_reserves_same in STEPS2; eauto.
+    unguard. des.
+    - eapply NORESERVES; eauto.
+    - rewrite PROMISES in *. erewrite Memory.bot_get in STEPS2. clarify. }
+
+  eapply hold_or_not with (Q := no_sc) in STEPS2. des.
+
+  - destruct e2. ss.
+    exploit no_sc_any_sc_rtc; try eapply HOLD; eauto.
+    { ss. i. des. auto. } i. des.
+    esplits.
+    + eapply pred_step_rtc_mon; try eapply STEP0. i. ss.
+    + ss. unguard. des.
+      * left. ss. inv FAILURE; inv STEP1. inv LOCAL. eauto.
+      * right. esplits; eauto.
+
+  - exploit Thread.rtc_tau_step_future.
+    { eapply thread_steps_pred_steps. eapply STEPS0. }
+    { ss. }
+    { ss. }
+    { ss. } i. des.
+    inv STEP0.
+    exploit Thread.step_future; eauto. i. des.
+
+    assert (PROMS: Local.promise_consistent e3.(Thread.local)).
+    { eapply rtc_tau_step_promise_consistent.
+      - eapply thread_steps_pred_steps. eapply STEPS1.
+      - unguard. des.
+        + inv FAILURE; inv STEP0. inv LOCAL. inv LOCAL0. ss.
+        + ii. rewrite PROMISES in PROMISE.
+          rewrite Memory.bot_get in PROMISE. clarify.
+      - eauto.
+      - eauto.
+      - eauto. }
+
+    assert (NOPROMISE: e2'.(Thread.local).(Local.promises) = Memory.bot).
+    { apply Memory.ext. i. rewrite Memory.bot_get.
+      destruct (Memory.get loc ts (Local.promises (Thread.local e2')))
+        as [[from [val released|]]|] eqn:GET; auto; cycle 1.
+      - exfalso.
+        eapply step_not_cancel_reserves_same in GET; cycle 1.
+        + econs.
+          * econs; eauto.
+          * instantiate (1:=promise_free /1\ (fun e => ~ is_cancel e)). ss.
+        + ss.
+        + des. eapply steps_not_cancel_reserves_same in GET; eauto.
+          des. eapply NORESERVES; eauto.
+      - exfalso.
+        exploit pf_step_rtc_promises_decrease.
+        { eapply STEPS0. }
+        { i. ss. des. auto. }
+        { econs; eauto. } ss. i.
+        exploit pf_step_rtc_promises_decrease.
+        { eapply STEP. }
+        { i. unfold is_cancel in *. des_ifs. }
+        { ss. eauto. }
+        ss. i. inv x2.
+        ss. unfold no_sc in BREAKQ. des_ifs; try by (exfalso; eauto).
+        + des; clarify. apply NNPP in BREAKQ.
+          inv STEP1; inv STEP0. ss. inv LOCAL. inv LOCAL0. ss.
+          eapply PROMS in GET. ss. des_ifs. ss.
+          hexploit max_concrete_timemap_get; eauto.
+          * inv WF. eapply Memory.cap_le; eauto.
+          * i. eapply Time.lt_strorder. eapply TimeFacts.lt_le_lt; eauto.
+        + inv STEP1; inv STEP0. ss. inv LOCAL. inv LOCAL0. ss.
+          eapply PROMS in GET. ss. des_ifs. ss.
+          hexploit max_concrete_timemap_get; eauto.
+          * inv WF. eapply Memory.cap_le; eauto.
+          * i. eapply Time.lt_strorder. eapply TimeFacts.lt_le_lt; eauto.
+    }
+
+    destruct e2'. destruct local. ss.
+    eapply no_sc_any_sc_rtc in STEPS0; ss; cycle 1.
+    { i. des; ss. } des.
+    esplits.
+    * eapply pred_step_rtc_mon; eauto. i. ss.
+    * unguard. ss. eauto.
+Qed.
+
+
+Inductive unattachable (mem: Memory.t) (loc: Loc.t) (ts: Time.t): Prop :=
+| unattachable_intro
+    to msg
+    (MSG: Memory.get loc to mem = Some (ts, msg))
+    (EMPTY: Memory.get loc ts mem = None)
+.
+
+Lemma lower_unattachable mem1 mem0 loc from to msg1 msg2
+      (LOWER: Memory.lower mem0 loc from to msg1 msg2 mem1)
+  :
+    unattachable mem1 = unattachable mem0.
+Proof.
+  extensionality loc0. extensionality ts0.
+  exploit Memory.lower_get0; eauto. i. des.
+  apply Coq.Logic.PropExtensionality.propositional_extensionality. split; i.
+  { inv H. erewrite Memory.lower_o in EMPTY; eauto.
+    erewrite Memory.lower_o in MSG; eauto. des_ifs.
+    { ss. des; clarify. econs; eauto. }
+    { econs; eauto. }
+  }
+  { inv H. eapply Memory.lower_get1 in MSG; eauto. des. econs; eauto.
+    erewrite Memory.lower_o; eauto. des_ifs. ss. des. clarify. }
+Qed.
+
+Lemma split_unattachable mem1 mem0 loc ts1 ts2 ts3 msg2 msg3
+      (SPLIT: Memory.split mem0 loc ts1 ts2 ts3 msg2 msg3 mem1)
+  :
+    unattachable mem1 = unattachable mem0.
+Proof.
+  extensionality loc0. extensionality ts0.
+  exploit split_succeed_wf; eauto. i. des.
+  exploit Memory.split_get0; eauto. i. des.
+  apply Coq.Logic.PropExtensionality.propositional_extensionality. split; i.
+  { inv H. erewrite Memory.split_o in MSG; eauto.
+    erewrite Memory.split_o in EMPTY; eauto. des_ifs.
+    { ss. des; clarify. econs; eauto. }
+    { ss. des; clarify. }
+    { econs; eauto. }
+  }
+  { inv H. generalize (Memory.split_o loc0 to SPLIT). intros MSG0. des_ifs.
+    { ss. des; clarify. }
+    { ss. des; clarify. econs; eauto.
+      erewrite Memory.split_o; eauto. des_ifs.
+      { ss. des; clarify. timetac. }
+      { ss. des; clarify. }
+    }
+    { econs.
+      { instantiate (2:=to).
+        erewrite Memory.split_o; eauto. des_ifs.
+        { ss. des; clarify. }
+        { ss. des; clarify. }
+        { eauto. }
+      }
+      { erewrite Memory.split_o; eauto. des_ifs.
+        { ss. des; clarify. exfalso.
+          exploit memory_get_from_inj.
+          { eapply GET3. }
+          { erewrite MSG0. eauto. }
+          i. des; clarify.
+        }
+        { ss. des; clarify. }
+      }
+    }
+  }
+Qed.
+
+Lemma add_unattachable mem1 mem0 loc from to msg
+      (ADD: Memory.add mem0 loc from to msg mem1)
+  :
+    unattachable mem1 =
+    (fun loc0 ts0 =>
+       if loc_ts_eq_dec (loc0, ts0) (loc, to) then False
+       else if loc_ts_eq_dec (loc0, ts0) (loc, from) then
+              match Memory.get loc from mem0 with
+              | Some _ => False
+              | None => True
+              end
+            else unattachable mem0 loc0 ts0).
+Proof.
+  extensionality loc0. extensionality ts0.
+  exploit add_succeed_wf; eauto. i.  des.
+  exploit Memory.add_get0; eauto. i. des.
+  apply Coq.Logic.PropExtensionality.propositional_extensionality. split; i.
+  { inv H. erewrite Memory.add_o in MSG; eauto.
+    erewrite Memory.add_o in EMPTY; eauto. des_ifs.
+    { ss. des; clarify. }
+    { ss. des; clarify. }
+    { ss. des; clarify. }
+    { econs; eauto. }
+  }
+  { des_ifs.
+    { ss. des; clarify. econs; eauto.
+      erewrite Memory.add_o; eauto. des_ifs. ss. des; clarify. }
+    { inv H. econs; eauto.
+      { eapply Memory.add_get1; eauto. }
+      { erewrite Memory.add_o; eauto. des_ifs. ss. des; clarify. }
+    }
+  }
+Qed.
+
+Lemma remove_unattachable mem1 mem0 loc from to msg
+      (REMOVE: Memory.remove mem0 loc from to msg mem1)
+      (TS: Time.lt from to)
+  :
+    unattachable mem1 =
+    (fun loc0 ts0 =>
+       if loc_ts_eq_dec (loc0, ts0) (loc, from) then False
+       else if loc_ts_eq_dec (loc0, ts0) (loc, to) then
+              exists ts' msg', (<<GET: Memory.get loc ts' mem0 = Some (to, msg')>>)
+            else unattachable mem0 loc0 ts0).
+Proof.
+  extensionality loc0. extensionality ts0.
+  exploit Memory.remove_get0; eauto. i. des.
+  apply Coq.Logic.PropExtensionality.propositional_extensionality. split; i.
+  { inv H. erewrite Memory.remove_o in MSG; eauto.
+    erewrite Memory.remove_o in EMPTY; eauto. des_ifs.
+    { ss. des; clarify. timetac. }
+    { ss. des; clarify. exploit memory_get_from_inj.
+      { eapply MSG. }
+      { eapply GET. }
+      i. des; clarify.
+    }
+    { ss. des; clarify. esplits; eauto. }
+    { econs; eauto. }
+  }
+  { des_ifs.
+    { ss. des; clarify. econs; eauto.
+      erewrite Memory.remove_o; eauto. des_ifs; eauto.
+      ss. des; clarify.
+    }
+    { ss. inv H. econs.
+      { instantiate (2:=to0). erewrite Memory.remove_o; eauto. des_ifs; eauto.
+        ss. des; clarify. }
+      { erewrite Memory.remove_o; eauto. des_ifs. }
+    }
+  }
+Qed.
+
+
+Lemma step_lifting_promise prom0 prom1 mem0 mem1 cap0
+      loc from to msg kind
+      (spaces lefts: Loc.t -> Time.t -> Prop)
+      (PROMISE: Memory.promise prom0 mem0 loc from to msg prom1 mem1 kind)
+      (WRITENOTIN: forall ts (ITV: Interval.mem (from, to) ts), ~ spaces loc ts)
+      (WRITENOTTO: ~ lefts loc to)
+      (SOUND: Memory.le mem0 cap0)
+      (SPACES:
+         forall loc ts (COV: covered loc ts cap0),
+           <<COV: covered loc ts mem0>> \/ <<SPACE: spaces loc ts>>)
+      (UNATTACHABLE:
+         forall loc ts (COV: unattachable cap0 loc ts),
+           <<COV: unattachable mem0 loc ts>> \/ <<LEFT: lefts loc ts>>)
+      (MEM0: Memory.closed mem0)
+      (PROM0: Memory.le prom0 mem0)
+      (PROM1: Memory.le prom0 cap0)
+      (NOTCANCEL: kind <> Memory.op_kind_cancel)
+  :
+    exists cap1,
+      (<<STEP: Memory.promise prom0 cap0 loc from to msg prom1 cap1 kind>>) /\
+      (<<SOUND: Memory.le mem1 cap1>>) /\
+      (<<SPACES:
+         forall loc ts (COV: covered loc ts cap1),
+           <<COV: covered loc ts mem1>> \/ spaces loc ts>>) /\
+      (<<UNATTACHABLE:
+         forall loc ts (COV: unattachable cap1 loc ts),
+           <<COV: unattachable mem1 loc ts>> \/ lefts loc ts>>).
+Proof.
+  inv PROMISE.
+  { exploit add_succeed_wf; try apply MEM; eauto. i. des.
+    exploit (@Memory.add_exists cap0 loc from to msg); eauto.
+    { ii. exploit SPACES.
+      { econs; eauto. }
+      i. des.
+      { inv COV. eapply DISJOINT; eauto. }
+      { eapply WRITENOTIN; eauto. }
+    }
+    i. des. esplits.
+    { econs; eauto. i. exploit UNATTACHABLE.
+      { econs; eauto. eapply Memory.add_get0; eauto. }
+      i. des.
+      { inv COV. eapply ATTACH; eauto. }
+      { eapply WRITENOTTO; eauto. }
+    }
+    { ii. erewrite Memory.add_o in LHS; eauto.
+      erewrite (@Memory.add_o mem2 cap0); eauto. des_ifs.
+      eapply SOUND; eauto. }
+    { i. erewrite add_covered in COV; eauto.
+      erewrite (@add_covered mem1 mem0); eauto. des; eauto.
+      eapply SPACES in COV. des; auto. }
+    { i. erewrite add_unattachable in COV; eauto.
+      erewrite (@add_unattachable mem1 mem0); eauto. des_ifs; eauto.
+      ss. des; clarify. destruct p. eapply SOUND in Heq. clarify. }
+  }
+  { des. subst.
+    exploit (@Memory.split_exists_le prom0 cap0); eauto. i. des. esplits.
+    { econs; eauto. }
+    { ii. erewrite Memory.split_o in LHS; eauto.
+      erewrite (@Memory.split_o mem2 cap0); eauto. des_ifs.
+      eapply SOUND; eauto. }
+    { i. erewrite (@split_covered mem2 cap0) in COV; eauto.
+      erewrite (@split_covered mem1 mem0); eauto. }
+    { i. erewrite (@split_unattachable mem2 cap0) in COV; eauto.
+      erewrite (@split_unattachable mem1 mem0); eauto. }
+  }
+  { des. subst.
+    exploit (@Memory.lower_exists_le prom0 cap0); eauto. i. des. esplits.
+    { econs; eauto. }
+    { ii. erewrite Memory.lower_o in LHS; eauto.
+      erewrite (@Memory.lower_o mem2 cap0); eauto. des_ifs.
+      eapply SOUND; eauto. }
+    { i. erewrite (@lower_covered mem2 cap0) in COV; eauto.
+      erewrite (@lower_covered mem1 mem0); eauto. }
+    { i. erewrite (@lower_unattachable mem2 cap0) in COV; eauto.
+      erewrite (@lower_unattachable mem1 mem0); eauto. }
+  }
+  { ss. }
+Qed.
+
+Lemma step_lifting lang st0 st1 lc0 lc1 sc0 sc1 mem0 mem1 cap0 pf e
+      (spaces lefts: Loc.t -> Time.t -> Prop)
+      (STEP: Thread.step pf e (Thread.mk lang st0 lc0 sc0 mem0) (Thread.mk _ st1 lc1 sc1 mem1))
+      (WRITENOTIN: write_not_in spaces e)
+      (WRITENOTTO: write_not_to lefts e)
+      (NOTCANCEL: ~ is_cancel e)
+      (SOUND: Memory.le mem0 cap0)
+      (SPACES:
+         forall loc ts (COV: covered loc ts cap0),
+           <<COV: covered loc ts mem0>> \/ <<SPACE: spaces loc ts>>)
+      (UNATTACHABLE:
+         forall loc ts (COV: unattachable cap0 loc ts),
+           <<COV: unattachable mem0 loc ts>> \/ <<LEFT: lefts loc ts>>)
+      (MEM0: Memory.closed mem0)
+      (LOCAL0: Local.wf lc0 mem0)
+      (SC0: Memory.closed_timemap sc0 mem0)
+  :
+    exists cap1,
+      (<<STEP: Thread.step pf e (Thread.mk _ st0 lc0 sc0 cap0) (Thread.mk _ st1 lc1 sc1 cap1)>>) /\
+      (<<SOUND: Memory.le mem1 cap1>>) /\
+      (<<SPACES:
+         forall loc ts (COV: covered loc ts cap1),
+           <<COV: covered loc ts mem1>> \/ spaces loc ts>>) /\
+      (<<UNATTACHABLE:
+         forall loc ts (COV: unattachable cap1 loc ts),
+           <<COV: unattachable mem1 loc ts>> \/ lefts loc ts>>).
+Proof.
+  inv STEP.
+  { inv STEP0. inv LOCAL. ss.
+    destruct (Memory.op_kind_is_cancel kind) eqn:KIND; ss.
+    { destruct kind; ss. }
+    exploit step_lifting_promise; eauto.
+    { eapply LOCAL0. }
+    { transitivity mem0; eauto. eapply LOCAL0. }
+    { destruct kind; ss. }
+    i. des. esplits; eauto. econs. econs.
+    { econs; eauto. eapply memory_concrete_le_closed_msg; eauto. }
+    { ss. destruct kind; ss. }
+  }
+  { inv STEP0. inv LOCAL.
+    { esplits; eauto. }
+    { inv LOCAL1. eapply SOUND in GET. esplits; eauto. }
+    { inv LOCAL1. inv WRITE. exploit step_lifting_promise; eauto.
+      { eapply LOCAL0. }
+      { transitivity mem0; eauto. eapply LOCAL0. }
+      { destruct kind; ss. inv PROMISE; ss. }
+      i. des. esplits; eauto. econs 2; eauto.
+    }
+    { inv LOCAL1. eapply SOUND in GET. inv LOCAL2. inv WRITE.
+      exploit step_lifting_promise; eauto.
+      { eapply LOCAL0. }
+      { transitivity mem0; eauto. eapply LOCAL0. }
+      { destruct kind; ss. inv PROMISE; ss. }
+      i. des. esplits; eauto. econs 2; eauto. econs; eauto. }
+    { esplits; eauto. }
+    { esplits; eauto. }
+    { esplits; eauto. }
+  }
+Qed.
+
+Lemma traced_step_lifting lang st0 st1 lc0 lc1 sc0 sc1 mem0 mem1 cap0 tr
+      (spaces lefts: Loc.t -> Time.t -> Prop)
+      (STEPS: Trace.steps tr (Thread.mk lang st0 lc0 sc0 mem0) (Thread.mk _ st1 lc1 sc1 mem1))
+      (EVENTS: List.Forall (fun em => <<SAT: (write_not_in spaces /1\ write_not_to lefts /1\ (fun e => ~ is_cancel e)) (snd em)>>) tr)
+      (SOUND: Memory.le mem0 cap0)
+      (SPACES:
+         forall loc ts (COV: covered loc ts cap0),
+           <<COV: covered loc ts mem0>> \/ <<SPACE: spaces loc ts>>)
+      (UNATTACHABLE:
+         forall loc ts (COV: unattachable cap0 loc ts),
+           <<COV: unattachable mem0 loc ts>> \/ <<LEFT: lefts loc ts>>)
+      (MEM0: Memory.closed mem0)
+      (LOCAL0: Local.wf lc0 mem0)
+      (SC0: Memory.closed_timemap sc0 mem0)
+  :
+    exists cap1,
+      (<<STEPS: Trace.steps tr (Thread.mk _ st0 lc0 sc0 cap0) (Thread.mk _ st1 lc1 sc1 cap1)>>) /\
+      (<<SOUND: Memory.le mem1 cap1>>) /\
+      (<<SPACES:
+         forall loc ts (COV: covered loc ts cap1),
+           <<COV: covered loc ts mem1>> \/ spaces loc ts>>) /\
+      (<<UNATTACHABLE:
+         forall loc ts (COV: unattachable cap1 loc ts),
+           <<COV: unattachable mem1 loc ts>> \/ lefts loc ts>>).
+Proof.
+  remember (Thread.mk lang st0 lc0 sc0 mem0).
+  remember (Thread.mk lang st1 lc1 sc1 mem1). ginduction STEPS.
+  { i. clarify. esplits; eauto. }
+  { i. clarify. inv EVENTS. ss. des.
+    exploit Thread.step_future; eauto. i. des.
+    destruct th1. ss. exploit step_lifting; eauto. i. des.
+    exploit IHSTEPS; eauto. i. des. exists cap2. splits; auto. econs; eauto.
+  }
+Qed.
+
+Lemma promise_not_cancel_covered_increase prom0 prom1 mem0 mem1
+      loc from to msg kind
+      (PROMISE: Memory.promise prom0 mem0 loc from to msg prom1 mem1 kind)
+      (NOTCANCEL: kind <> Memory.op_kind_cancel)
+      loc0 ts0
+      (COVERED: covered loc0 ts0 mem0)
+  :
+    covered loc0 ts0 mem1.
+Proof.
+  inv PROMISE.
+  { erewrite (@add_covered mem1 mem0); eauto. }
+  { erewrite (@split_covered mem1 mem0); eauto. }
+  { erewrite (@lower_covered mem1 mem0); eauto. }
+  { ss. }
+Qed.
+
+Lemma step_not_cancel_covered_increase lang (th0 th1: Thread.t lang) pf e
+      (STEP: Thread.step pf e th0 th1)
+      (NOTCANCEL: ~ is_cancel e)
+      loc0 ts0
+      (COVERED: covered loc0 ts0 th0.(Thread.memory))
+  :
+    covered loc0 ts0 th1.(Thread.memory).
+Proof.
+  inv STEP.
+  { inv STEP0. inv LOCAL. ss.
+    eapply promise_not_cancel_covered_increase; eauto. destruct kind; ss.
+  }
+  { inv STEP0. inv LOCAL; auto.
+    { inv LOCAL0. inv WRITE. eapply promise_not_cancel_covered_increase; eauto.
+      destruct kind; ss. inv PROMISE; ss. }
+    { inv LOCAL2. inv WRITE. eapply promise_not_cancel_covered_increase; eauto.
+      destruct kind; ss. inv PROMISE; ss. }
+  }
+Qed.
+
+Lemma traced_steps_not_cancel_covered_increase lang (th0 th1: Thread.t lang) tr
+      (STEPS: Trace.steps tr th0 th1)
+      (EVENTS: List.Forall (fun em => <<SAT: (fun e => ~ is_cancel e) (snd em)>>) tr)
+      loc0 ts0
+      (COVERED: covered loc0 ts0 th0.(Thread.memory))
+  :
+    covered loc0 ts0 th1.(Thread.memory).
+Proof.
+  ginduction STEPS; auto. i. clarify. inv EVENTS.
+  eapply step_not_cancel_covered_increase in STEP; eauto.
+Qed.
+
+Inductive reservations_added:
+  forall (l: list (Loc.t * Interval.t)) (mem0 mem1: Memory.t), Prop :=
+| reservations_added_base
+    mem0
+  :
+    reservations_added [] mem0 mem0
+| reservations_added_cons
+    mem0 mem1 mem2 loc from to tl
+    (ADD: Memory.add mem0 loc from to Message.reserve mem1)
+    (TL: reservations_added tl mem1 mem2)
+    (WF: Time.lt from to)
+  :
+    reservations_added ((loc, (from, to))::tl) mem0 mem2
+.
+
+Lemma reservations_added_cancel
+      loc from to mem0 mem1 mem2 tl
+      (CANCEL: Memory.remove mem1 loc from to Message.reserve mem0)
+      (TL: reservations_added tl mem1 mem2)
+      (WF: Time.lt from to)
+  :
+    reservations_added ((loc, (from, to))::tl) mem0 mem2.
+Proof.
+  econs; eauto.
+  exploit (@Memory.add_exists mem0 loc from to Message.reserve); eauto.
+  { i. erewrite Memory.remove_o in GET2; eauto. des_ifs.
+    exploit Memory.get_disjoint.
+    { eapply GET2. }
+    { eapply Memory.remove_get0; eauto. }
+    i. ss. des; clarify. symmetry. auto.
+  }
+  { econs. }
+  i. des. replace mem1 with mem3; auto. eapply Memory.ext.
+  i. erewrite (@Memory.add_o mem3 mem0); eauto.
+  erewrite (@Memory.remove_o mem0 mem1); eauto. des_ifs.
+  ss. des; clarify. symmetry. eapply Memory.remove_get0; eauto.
+Qed.
+
+Lemma remove_covered_unattachable mem0 loc from to msg mem1
+      (REMOVE: Memory.remove mem0 loc from to msg mem1)
+      (CLOSED: Memory.closed mem0)
+      (TS: Time.lt from to)
+  :
+    (<<COVERED: forall ts (ITV: Interval.mem (from, to) ts), ~ covered loc ts mem1>>) /\
+    (<<UNATTACHABLE: forall ts (TS0: Time.le from ts) (TS1: Time.lt ts to),
+        ~ unattachable mem1 loc ts>>).
+Proof.
+  exploit Memory.remove_get0; eauto. i. des. split.
+  { ii. inv H. erewrite Memory.remove_o in GET1; eauto. des_ifs.
+    exploit Memory.get_disjoint.
+    { eapply GET1. }
+    { eapply GET. }
+    i. des; clarify. eapply x0; eauto.
+  }
+  { ii. inv H. erewrite Memory.remove_o in MSG; eauto.
+    erewrite Memory.remove_o in EMPTY; eauto. des_ifs.
+    { ss. des; clarify. timetac. }
+    exploit Memory.get_disjoint.
+    { eapply MSG. }
+    { eapply GET. }
+    i. ss. des; clarify.
+    eapply memory_get_ts_strong in MSG. des; clarify.
+    { inv CLOSED. erewrite INHABITED in EMPTY. ss. }
+    eapply x0.
+    { instantiate (1:=Time.meet to to0). unfold Time.meet. des_ifs.
+      econs; ss. refl.
+    }
+    { unfold Time.meet. des_ifs.
+      { econs; ss. refl. }
+      { econs; ss.
+        { eapply TimeFacts.le_lt_lt; eauto. }
+        { left. auto. }
+      }
+    }
+  }
+Qed.
+
+Fixpoint intervals_sum (l: list (Loc.t * Interval.t)):
+  Loc.t -> Time.t -> Prop :=
+  match l with
+  | [] => bot2
+  | (loc, (from, to))::tl =>
+    fun loc0 ts0 =>
+      (loc0 = loc /\ Interval.mem (from, to) ts0) \/
+      intervals_sum tl loc0 ts0
+  end.
+
+Definition is_reserving (te: ThreadEvent.t): Prop :=
+  match te with
+  | ThreadEvent.promise _ _ _ Message.reserve Memory.op_kind_add => True
+  | _ => False
+  end.
+
+Lemma reservations_added_cancelable l prom0 prom1 cap1
+      (ADDEDPROM: reservations_added l prom0 prom1)
+      (WF: Memory.le prom1 cap1)
+      (CLOSED: Memory.closed cap1)
+  :
+    exists cap0,
+      (<<FUTURE: reservations_added l cap0 cap1>>) /\
+      (<<COVERED: forall loc ts
+                         (ITV: intervals_sum l loc ts),
+          ~ covered loc ts cap0>>) /\
+      (* (<<UNATTACHABLE: forall loc from to ts *)
+      (*                         (IN: List.In (loc, (from, to)) l) *)
+      (*                         (TS0: Time.le from ts) *)
+      (*                         (TS1: Time.lt ts to), *)
+      (*     ~ unattachable cap0 loc ts>>) /\ *)
+      (<<MLE: Memory.le prom0 cap0>>) /\
+      (<<SOUND: forall loc ts (NIN: forall from, ~ List.In (loc, (from, ts)) l),
+          Memory.get loc ts cap0 = Memory.get loc ts cap1>>) /\
+      (<<CLOSED: Memory.closed cap0>>)
+.
+Proof.
+  ginduction l.
+  { i. inv ADDEDPROM. exists cap1. splits; eauto.
+    { econs 1. }
+  }
+  { i. inv ADDEDPROM.
+    exploit IHl; eauto. i. des.
+    hexploit (@Memory.remove_exists mem1 loc from to Message.reserve).
+    { eapply Memory.add_get0; eauto. }
+    i. des.
+    hexploit MemoryMerge.add_remove.
+    { eapply ADD. }
+    { eapply H. } i. subst.
+    hexploit (@Memory.remove_exists_le mem1 cap0); eauto. i. des.
+    exploit remove_covered_unattachable; try apply H0; eauto. i. des.
+    esplits.
+    { eapply reservations_added_cancel; eauto. }
+    { i. ss. des; subst; eauto.
+      eapply COVERED in ITV; eauto.
+      erewrite remove_covered; eauto. ii. eapply ITV. des; auto.
+    }
+    { ii. erewrite (@Memory.remove_o mem2 mem1) in LHS; eauto.
+      erewrite (@Memory.remove_o mem0 cap0); eauto. des_ifs.
+      eapply MLE; eauto.
+    }
+    { i. erewrite (@Memory.remove_o mem0 cap0); eauto. des_ifs.
+      { ss. des; clarify. exfalso. eapply NIN; eauto. }
+      { eapply SOUND; eauto. ii. eapply NIN; ss. right. eauto. }
+    }
+    { eapply Memory.cancel_closed; eauto. }
+  }
+Qed.
+
+Lemma promise_needed_spaces prom0 prom1 mem0 mem1
+      loc from to msg kind
+      (PROMISE: Memory.promise prom0 mem0 loc from to msg prom1 mem1 kind)
+      (WF: kind <> Memory.op_kind_cancel)
+  :
+    ((<<ALREADY: forall ts (ITV: Interval.mem (from, to) ts), covered loc ts mem0>>) /\
+     (<<COVERED: forall loc ts, covered loc ts mem1 <-> covered loc ts mem0>>))
+    \/
+    ((<<NEW: forall ts (ITV: Interval.mem (from, to) ts), ~ covered loc ts mem0>>) /\
+     (<<COVERED: forall loc0 ts0 (COV: covered loc0 ts0 mem1),
+         covered loc0 ts0 mem0 \/ (loc0 = loc /\ Interval.mem (from, to) ts0)>>) /\
+     (<<WF: Time.lt from to>>))
+.
+Proof.
+  inv PROMISE.
+  { right. exploit add_succeed_wf; try apply MEM. i. des. splits; auto.
+    { ii. inv H. eapply DISJOINT; eauto. }
+    { i. erewrite add_covered in COV; eauto. }
+  }
+  { left. exploit split_succeed_wf; try apply MEM. i. des. splits; auto.
+    { ii. econs; eauto. eapply Interval.le_mem; eauto. econs; ss.
+      { refl. }
+      { left. auto. }
+    }
+    { i. eapply split_covered; eauto. }
+  }
+  { left. exploit lower_succeed_wf; try apply MEM. i. des. splits; auto.
+    { ii. econs; eauto. }
+    { i. eapply lower_covered; eauto. }
+  }
+  { ss. }
+Qed.
+
+Lemma step_needed_spaces lang (th0 th1: Thread.t lang) pf e
+      (times: Loc.t -> Time.t -> Prop)
+      (STEP: Thread.step pf e th0 th1)
+      (NOTCANCEL: ~ is_cancel e)
+      (WFTIME: wf_time_evt times e)
+  :
+    ((<<ALREADY: write_not_in (fun loc0 ts0 => ~ covered loc0 ts0 th0.(Thread.memory)) e>>) /\
+     (<<COVERED: forall loc ts, covered loc ts th1.(Thread.memory) <-> covered loc ts th0.(Thread.memory)>>))
+    \/
+    exists loc from to,
+      (<<NEW: forall ts (ITV: Interval.mem (from, to) ts), ~ covered loc ts th0.(Thread.memory)>>) /\
+      (<<COVERED: forall loc0 ts0 (COV: covered loc0 ts0 th1.(Thread.memory)),
+          covered loc0 ts0 th0.(Thread.memory) \/ (loc0 = loc /\ Interval.mem (from, to) ts0)>>) /\
+      (<<WF: Time.lt from to>>) /\
+      (<<TIMES: times loc from /\ times loc to>>) /\
+      (<<EVENT: write_not_in (fun loc0 ts0 => ~ (loc0 = loc /\ Interval.mem (from, to) ts0)) e>>).
+Proof.
+  inv STEP.
+  { inv STEP0. inv LOCAL. ss.
+    destruct (Memory.op_kind_is_cancel kind) eqn:KIND.
+    { destruct kind; ss. }
+    exploit promise_needed_spaces; eauto.
+    { destruct kind; ss. }
+    i. des.
+    { left. splits; auto. }
+    { right. esplits; eauto. }
+  }
+  { inv STEP0. inv LOCAL; try by (splits; eauto); ss.
+    { ss. inv LOCAL0. inv WRITE.
+      exploit promise_needed_spaces; eauto.
+      { destruct kind; ss. inv PROMISE; ss. }
+      i. des.
+      { left. esplits; eauto. }
+      { right. esplits; eauto. }
+    }
+    { ss. inv LOCAL2. inv WRITE.
+      exploit promise_needed_spaces; eauto.
+      { destruct kind; ss. inv PROMISE; ss. }
+      i. des.
+      { left. esplits; eauto. }
+      { right. esplits; eauto. }
+    }
+  }
+Qed.
+
+Inductive added_intervals
+  :
+    forall (l: list (Loc.t * Interval.t)) (mem0 mem1: Memory.t), Prop :=
+| added_intervals_base
+    mem0 mem1
+    (COVERED: forall loc ts, covered loc ts mem1 <-> covered loc ts mem0)
+  :
+    added_intervals [] mem0 mem1
+| added_intervals_cons
+    mem0 mem1 mem2
+    loc from to tl
+    (TL: added_intervals tl mem1 mem2)
+    (NCOV: forall ts (ITV: Interval.mem (from, to) ts), ~ covered loc ts mem0)
+    (COV: forall loc0 ts0 (COVERED: covered loc0 ts0 mem1),
+        covered loc0 ts0 mem0 \/ (loc0 = loc /\ Interval.mem (from, to) ts0))
+    (TS: Time.lt from to)
+  :
+    added_intervals ((loc, (from, to)) :: tl) mem0 mem2
+.
+Hint Constructors added_intervals.
+
+Lemma added_intervals_sum l mem0 mem1
+      (ADDED: added_intervals l mem0 mem1)
+      loc ts
+      (COV: covered loc ts mem1)
+  :
+    covered loc ts mem0 \/ intervals_sum l loc ts.
+Proof.
+  ginduction ADDED; i; ss.
+  { erewrite <- COVERED; eauto. }
+  { exploit IHADDED; eauto. i. des; auto.
+    exploit COV; eauto. i. des; auto. }
+Qed.
+
+Lemma same_covered_added_intervals l mem0 mem1 mem2
+      (ADDED: added_intervals l mem0 mem2)
+      (COVERED: forall loc ts, covered loc ts mem1 <-> covered loc ts mem0)
+  :
+    added_intervals l mem1 mem2.
+Proof.
+  ginduction ADDED; i; eauto.
+  { econs. i. erewrite COVERED0. auto. }
+  { econs; eauto.
+    { i. erewrite COVERED; eauto. }
+    { i. erewrite COVERED; eauto. }
+  }
+Qed.
+
+Lemma traced_steps_needed_spaces lang (th0 th1: Thread.t lang) tr
+      (times: Loc.t -> Time.t -> Prop)
+      (STEP: Trace.steps tr th0 th1)
+      (EVENTS: List.Forall (fun em => <<SAT: ((fun e => ~ is_cancel e) /1\ wf_time_evt times) (snd em)>>) tr)
+  :
+    exists l,
+      (<<WRITENOTIN:
+         List.Forall (fun em => <<SAT: write_not_in (fun loc ts => ~ (covered loc ts th0.(Thread.memory) \/ intervals_sum l loc ts)) (snd em)>>) tr>>) /\
+      (<<WF: added_intervals l th0.(Thread.memory) th1.(Thread.memory)>>) /\
+      (<<TIMES: List.Forall (fun locitv =>
+                               times (fst locitv) (fst (snd locitv)) /\
+                               times (fst locitv) (snd (snd locitv))) l>>)
+.
+Proof.
+  ginduction STEP; i.
+  { i. exists []. splits; auto. }
+  { subst. inv EVENTS. des. exploit IHSTEP; eauto. i. des.
+    exploit step_needed_spaces; eauto. i. des.
+    { exists l. splits; auto.
+      { econs; eauto.
+        { eapply write_not_in_mon; eauto. i. ss.
+          eapply not_or_and in PR. des. auto. }
+        { eapply List.Forall_impl; eauto. i. ss.
+          eapply write_not_in_mon; eauto. i. ss.
+          erewrite COVERED. auto. }
+      }
+      { eapply same_covered_added_intervals; eauto.
+        i. erewrite COVERED; eauto. }
+    }
+    { exists ((loc, (from, to)) :: l). splits.
+      { econs.
+        { eapply write_not_in_mon; eauto. ss. i.
+          ii. des. eapply PR. eauto. }
+         { eapply List.Forall_impl; try apply WRITENOTIN; eauto. i. ss.
+           eapply write_not_in_mon; eauto. i. ss.
+           ii. eapply PR. des; auto. eapply COVERED in H3. des; auto. }
+      }
+      { econs; eauto. }
+      { econs; ss. }
+    }
+  }
+Qed.
+
+
+Lemma can_reserve_all_needed times
+      (DIVERGE: forall loc ts,
+          exists ts',
+            (<<TIMES: times loc ts'>>) /\
+            (<<TS: Time.lt ts ts'>>))
+      lang
+      st0 st1 lc0 lc1 sc0 sc1 mem0 mem1 tr
+      (MWF: memory_times_wf times mem0)
+      (STEPS: Trace.steps tr (Thread.mk lang st0 lc0 sc0 mem0) (Thread.mk lang st1 lc1 sc1 mem1))
+      (EVENTS: List.Forall (fun em => <<SAT: ((fun e => ~ is_cancel e) /1\ wf_time_evt times) (snd em)>>) tr)
+      (MEM: Memory.closed mem0)
+      (LOCAL: Local.wf lc0 mem0)
+      (SC: Memory.closed_timemap sc0 mem0)
+  :
+    exists lc0' mem0' tr_reserve tr_cancel,
+      (<<RESERVESTEPS:
+         Trace.steps tr_reserve (Thread.mk lang st0 lc0 sc0 mem0) (Thread.mk lang st0 lc0' sc0 mem0)>>) /\
+      (<<RESERVETRACE:
+         List.Forall (fun em => <<SAT: (is_reserving /1\ wf_time_evt times) (snd em)>>) tr_reserve>>) /\
+      (<<CANCELTRACE:
+         List.Forall (fun em => <<SAT: (is_cancel /1\ wf_time_evt times) (snd em)>>) tr_cancel>>) /\
+      (<<CAP:
+         forall cap0
+                (MLE: Memory.le mem0' cap0),
+         exists cap1,
+           (<<CANCELSTEPS:
+              Trace.steps tr_cancel (Thread.mk lang st0 lc0' sc0 cap0) (Thread.mk lang st0 lc0 sc0 mem0)>>) /\
+           (<<STEPS:
+              Trace.steps tr (Thread.mk lang st0 lc0 sc0 mem0) (Thread.mk lang st1 lc1 sc1 cap1)>>)>>).
+
+
+Lemma can_reserve_all_needed times
+      (DIVERGE: forall loc ts,
+          exists ts',
+            (<<TIMES: times loc ts'>>) /\
+            (<<TS: Time.lt ts ts'>>))
+      lang
+      st0 st1 tvw0 tvw1 prom0 prom1 sc0 sc1 mem0 mem1 tr
+      (MWF: memory_times_wf times mem0)
+      (STEPS: Trace.steps tr (Thread.mk lang st0 (Local.mk tvw0 prom0) sc0 mem0) (Thread.mk lang st1 (Local.mk tvw1 prom1) sc1 mem1))
+      (EVENTS: List.Forall (fun em => <<SAT: ((fun e => ~ is_cancel e) /1\ wf_time_evt times) (snd em)>>) tr)
+      (MEM: Memory.closed mem0)
+      (LOCAL: Local.wf (Local.mk tvw0 prom0) mem0)
+      (SC: Memory.closed_timemap sc0 mem0)
+  :
+    exists prom0' mem0' tr_reserve tr_cancel,
+      (<<RESERVESTEPS:
+         Trace.steps tr_reserve (Thread.mk lang st0 (Local.mk tvw0 prom0) sc0 mem0) (Thread.mk lang st0 (Local.mk tvw0 prom0') sc0 mem0)>>) /\
+      (<<RESERVETRACE:
+         List.Forall (fun em => <<SAT: (is_reserving /1\ wf_time_evt times) (snd em)>>) tr_reserve>>) /\
+      (<<CANCELTRACE:
+         List.Forall (fun em => <<SAT: (is_cancel /1\ wf_time_evt times) (snd em)>>) tr_cancel>>) /\
+      (<<CAP:
+         forall cap0
+                (MLE: Memory.le mem0' cap0),
+         exists cap1,
+           (<<CANCELSTEPS:
+              Trace.steps tr_cancel (Thread.mk lang st0 (Local.mk tvw0 prom0') sc0 cap0) (Thread.mk lang st0 (Local.mk tvw0 prom0) sc0 mem0)>>) /\
+           (<<STEPS:
+              Trace.steps tr (Thread.mk lang st0 (Local.mk tvw0 prom0) sc0 mem0) (Thread.mk lang st1 (Local.mk tvw1 prom1) sc1 cap1)>>)>>).
+
+           (<<CANCELSTEPS:
+              Trace.steps tr_cancel (Thread.mk lang st0 (Local.mk tvw0 prom0') sc0 cap0) (Thread.mk lang st0 (Local.mk tvw0 prom0') sc0 mem0)>>) /\
+
+
+
+                                                                                             cap0
+      (MLE: Memory.le mem0 cap0)
+
+
+
+      (<<RESERVEPROM: reservations_added l prom0 prom0'>>) /\
+      (<<RESERVEMEM: reservations_added l mem0 mem0'>>) /\
+
+
+Lemma can_reserve_needed times lang
+      st0 st1 tvw0 tvw1 prom0 prom1 sc0 sc1 mem0 mem1 tr
+      (MWF: memory_times_wf times mem0)
+      (STEPS: Trace.steps tr (Thread.mk lang st0 (Local.mk tvw0 prom0) sc0 mem0) (Thread.mk lang st1 (Local.mk tvw1 prom1) sc1 mem1))
+      (EVENTS: List.Forall (fun em => <<SAT: ((fun e => ~ is_cancel e) /1\ wf_time_evt times) (snd em)>>) tr)
+      (MEM: Memory.closed mem0)
+      (LOCAL: Local.wf (Local.mk tvw0 prom0) mem0)
+      (SC: Memory.closed_timemap sc0 mem0)
+  :
+    exists l prom0' mem0',
+      (<<RESERVEPROM: reservations_added l prom0 prom0'>>) /\
+      (<<RESERVEMEM: reservations_added l mem0 mem0'>>) /\
+
+
+
+         reserve_future_memory
+
+      (STEPS: Trace.steps tr (Thread.mk lang st0 lc0 sc0 mem0) (Thread.mk _ st1 lc1 sc1 mem1))
+      (EVENTS: List.Forall (fun em => <<SAT: (write_not_in spaces /1\ write_not_to lefts /1\ (fun e => ~ is_cancel e)) (snd em)>>) tr)
+      (SOUND: Memory.le mem0 cap0)
+      (SPACES:
+         forall loc ts (COV: covered loc ts cap0),
+           <<COV: covered loc ts mem0>> \/ <<SPACE: spaces loc ts>>)
+      (UNATTACHABLE:
+         forall loc ts (COV: unattachable cap0 loc ts),
+           <<COV: unattachable mem0 loc ts>> \/ <<LEFT: lefts loc ts>>)
+      (MEM0: Memory.closed mem0)
+      (LOCAL0: Local.wf lc0 mem0)
+      (SC0: Memory.closed_timemap tm0 mem0)
+
+
+  :
+
+
+
+
+
+
+
+      eapply
+
+        i.
+
+        eapply same_covered_added_intervals; eauto.
+        i. erewrite COVERED; eauto. }
+    }
+
+          eapply not_or_and in PR. des.
+
+
+
+          ii. eapply PR. des; auto.
+
+
+          eapply added_intervals_sum; eauto.
+
+          right.
+
+
+          eapply COVERED0; eauto. }
+      }
+      { auto.
+
+
+
+Lemma wf_empty_intervals_wf spaces mem l
+      (WF: wf_empty_intervals spaces mem l)
+      loc from to
+      (IN: List.In (loc, (from, to)) l)
+  :
+    (<<SPACES: forall ts (ITV: Interval.mem (from, to) ts), ~ spaces loc ts>>) /\
+    (<<TS: Time.lt from to>>).
+Proof.
+  ginduction l; ss. i. inv WF. des; clarify; eauto.
+Qed.
+
+Inductive intervals_sum (l: list (Loc.t * Interval.t))
+          (loc: Loc.t) (ts: Time.t): Prop :=
+| intervals_sum_intro
+    from to
+    (IN: List.In (loc, (from, to)) l)
+    (ITV: Interval.mem (from, to) ts)
+.
+Hint Constructors intervals_sum.
+
+Lemma wf_empty_intervals_sum spaces mem l
+      (WF: wf_empty_intervals spaces mem l)
+      loc ts
+      (ITV: intervals_sum l loc ts)
+  :
+    ~ spaces loc ts.
+Proof.
+  inv ITV. eapply wf_empty_intervals_wf; eauto.
+Qed.
+
+
+Lemma traced_steps_needed_spaces lang (th0 th1: Thread.t lang) tr
+      (spaces: Loc.t -> Time.t -> Prop)
+      (STEP: Trace.steps tr th0 th1)
+      (EVENTS: List.Forall (fun em => <<SAT: ((fun e => ~ is_cancel e) /1\ write_not_in spaces) (snd em)>>) tr)
+  (* (MEM0: Memory.closed mem0) *)
+  (* (LOCAL0: Local.wf lc0 mem0) *)
+  (* (SC0: Memory.closed_timemap tm0 mem0) *)
+  :
+    exists l,
+      (<<COVERED: forall loc0 ts0 (ITV: intervals_sum l loc0 ts0),
+          covered loc0 ts0 th1.(Thread.memory)>>) /\
+      (<<WRITENOTIN:
+         List.Forall (fun em => write_not_in (fun loc ts => ~ (intervals_sum l loc ts \/ covered loc ts th0.(Thread.memory))) (snd em)) tr>>) /\
+      (<<WF: wf_empty_intervals spaces th0.(Thread.memory) l>>)
+.
+Proof.
+  ginduction STEP; i.
+  { i. exists []. splits; auto. i. inv ITV. ss. }
+  { subst. inv EVENTS. des. exploit IHSTEP; eauto. i. des.
+    exploit step_needed_spaces; eauto. i. des.
+    { exists l. splits; auto.
+      { econs; eauto.
+        { eapply write_not_in_mon; eauto. i. ss.
+          eapply not_or_and in PR. des. auto. }
+        { eapply List.Forall_impl; eauto. i. ss.
+          eapply write_not_in_mon; eauto. i. ss.
+          ii. eapply PR. des; auto. right.
+          eapply COVERED0; eauto. }
+      }
+      { auto.
+
+
+           eapply not_or_and in PR. des. auto. }
+        {
+          eapply write
+        ss.
+
+
+
+  inv STEP.
+  { inv STEP0. inv LOCAL. ss.
+    destruct (Memory.op_kind_is_cancel kind) eqn:KIND; ss.
+    { destruct kind; ss. }
+    exploit promise_needed_spaces; eauto.
+    { destruct kind; ss. }
+    i. des.
+    {
+
+
+Lemma promise_needed_spaces_list prom0 prom1 mem0 mem1 l
+      loc from to msg kind
+      (spaces: Loc.t -> Time.t -> Prop)
+      (PROMISE: Memory.promise prom0 mem0 loc from to msg prom1 mem1 kind)
+      (WRITENOTIN: forall ts (ITV: Interval.mem (from, to) ts), ~ spaces loc ts)
+      (NOTCANCEL: kind <> Memory.op_kind_cancel)
+      (WFLIST: wf_empty_intervals spaces mem1 l)
+  :
+    exists l',
+      (<<WF: wf_empty_intervals spaces mem0 l>>) /\
+      (<<COVERED: forall loc0 ts0 (ITV: intervals_sum l loc0 ts0),
+          covered loc0 ts0 mem1>>) /\
+      (<<WRITENOTIN: forall ts (ITV: Interval.mem (from, to) ts),
+          (<<ALREADY: covered loc ts mem0>>) \/ (<<NEW: intervals_sum l loc ts>>)>>).
+Proof.
+  exploit promise_needed_spaces; eauto. i. des.
+  { exists []. splits.
+    { econs. }
+    { i. inv ITV. ss. }
+    { i. left. exploit promise_not_cancel_covered_increase; eauto. }
+  }
+  { exists [(loc, (from, to))]. splits; eauto.
+    { i. inv ITV; ss. des; clarify. eapply NEW; eauto. }
+    { i. right. econs; eauto. ss. auto. }
+  }
+Qed.
+
+Lemma promise_needed_spaces_list prom0 prom1 mem0 mem1
+      loc from to msg kind
+      (spaces: Loc.t -> Time.t -> Prop)
+      (PROMISE: Memory.promise prom0 mem0 loc from to msg prom1 mem1 kind)
+      (WRITENOTIN: forall ts (ITV: Interval.mem (from, to) ts), ~ spaces loc ts)
+      (WF: kind <> Memory.op_kind_cancel)
+  :
+    exists l,
+      (<<WF: wf_empty_intervals spaces mem0 l>>) /\
+      (<<COVERED: forall loc0 ts0 (ITV: intervals_sum l loc0 ts0),
+          covered loc0 ts0 mem1>>) /\
+      (<<WRITENOTIN: forall ts (ITV: Interval.mem (from, to) ts),
+          (<<ALREADY: covered loc ts mem0>>) \/ (<<NEW: intervals_sum l loc ts>>)>>).
+Proof.
+  exploit promise_needed_spaces; eauto. i. des.
+  { exists []. splits.
+    { econs. }
+    { i. inv ITV. ss. }
+    { i. left. exploit promise_not_cancel_covered_increase; eauto. }
+  }
+  { exists [(loc, (from, to))]. splits; eauto.
+    { i. inv ITV; ss. des; clarify. eapply NEW; eauto. }
+    { i. right. econs; eauto. ss. auto. }
+  }
+Qed.
+
+Lemma step_needed_spaces lang st0 st1 lc0 lc1 tm0 tm1 mem0 mem1 pf e
+      (spaces: Loc.t -> Time.t -> Prop)
+      (STEP: Thread.step pf e (Thread.mk lang st0 lc0 tm0 mem0) (Thread.mk _ st1 lc1 tm1 mem1))
+      (WRITENOTIN: write_not_in spaces e)
+      (NOTCANCEL: ~ is_cancel e)
+      (MEM0: Memory.closed mem0)
+      (LOCAL0: Local.wf lc0 mem0)
+      (SC0: Memory.closed_timemap tm0 mem0)
+  :
+    exists l,
+      (<<COVERED: forall loc0 ts0 (ITV: intervals_sum l loc0 ts0),
+          covered loc0 ts0 mem1>>) /\
+      (<<WRITENOTIN: forall ts (ITV: Interval.mem (from, to) ts),
+          (<<ALREADY: covered loc ts mem0>>) \/ (<<NEW: intervals_sum l loc ts>>)>>)      (<<WF: wf_empty_intervals spaces mem0 l>>)
+.
+Proof.
+  inv STEP.
+  { inv STEP0. inv LOCAL. ss.
+    destruct (Memory.op_kind_is_cancel kind) eqn:KIND; ss.
+    { destruct kind; ss. }
+    exploit promise_needed_spaces; eauto.
+    { destruct kind; ss. }
+    i. des.
+    {
+
+  }
+
+    exploit step_lifting_promise; eauto.
+    { eapply LOCAL0. }
+    { transitivity mem0; eauto. eapply LOCAL0. }
+    { destruct kind; ss. }
+    i. des. esplits; eauto. econs. econs.
+    { econs; eauto. eapply memory_concrete_le_closed_msg; eauto. }
+    { ss. destruct kind; ss. }
+  }
+  { inv STEP0. inv LOCAL.
+    { esplits; eauto. }
+    { inv LOCAL1. eapply SOUND in GET. esplits; eauto. }
+    { inv LOCAL1. inv WRITE. exploit step_lifting_promise; eauto.
+      { eapply LOCAL0. }
+      { transitivity mem0; eauto. eapply LOCAL0. }
+      { destruct kind; ss. inv PROMISE; ss. }
+      i. des. esplits; eauto. econs 2; eauto.
+    }
+    { inv LOCAL1. eapply SOUND in GET. inv LOCAL2. inv WRITE.
+      exploit step_lifting_promise; eauto.
+      { eapply LOCAL0. }
+      { transitivity mem0; eauto. eapply LOCAL0. }
+      { destruct kind; ss. inv PROMISE; ss. }
+      i. des. esplits; eauto. econs 2; eauto. econs; eauto. }
+    { esplits; eauto. }
+    { esplits; eauto. }
+    { esplits; eauto. }
+  }
+Qed.
+
+    exists cap1,
+      (<<STEP: Thread.step pf e (Thread.mk _ st0 lc0 tm0 cap0) (Thread.mk _ st1 lc1 tm1 cap1)>>) /\
+      (<<SOUND: Memory.le mem1 cap1>>) /\
+      (<<SPACES:
+         forall loc ts (COV: covered loc ts cap1),
+           <<COV: covered loc ts mem1>> \/ spaces loc ts>>) /\
+      (<<UNATTACHABLE:
+         forall loc ts (COV: unattachable cap1 loc ts),
+           <<COV: unattachable mem1 loc ts>> \/ lefts loc ts>>).
+Proof.
+  inv STEP.
+  { inv STEP0. inv LOCAL. ss.
+    destruct (Memory.op_kind_is_cancel kind) eqn:KIND; ss.
+    { destruct kind; ss. }
+    exploit step_lifting_promise; eauto.
+    { eapply LOCAL0. }
+    { transitivity mem0; eauto. eapply LOCAL0. }
+    { destruct kind; ss. }
+    i. des. esplits; eauto. econs. econs.
+    { econs; eauto. eapply memory_concrete_le_closed_msg; eauto. }
+    { ss. destruct kind; ss. }
+  }
+  { inv STEP0. inv LOCAL.
+    { esplits; eauto. }
+    { inv LOCAL1. eapply SOUND in GET. esplits; eauto. }
+    { inv LOCAL1. inv WRITE. exploit step_lifting_promise; eauto.
+      { eapply LOCAL0. }
+      { transitivity mem0; eauto. eapply LOCAL0. }
+      { destruct kind; ss. inv PROMISE; ss. }
+      i. des. esplits; eauto. econs 2; eauto.
+    }
+    { inv LOCAL1. eapply SOUND in GET. inv LOCAL2. inv WRITE.
+      exploit step_lifting_promise; eauto.
+      { eapply LOCAL0. }
+      { transitivity mem0; eauto. eapply LOCAL0. }
+      { destruct kind; ss. inv PROMISE; ss. }
+      i. des. esplits; eauto. econs 2; eauto. econs; eauto. }
+    { esplits; eauto. }
+    { esplits; eauto. }
+    { esplits; eauto. }
+  }
+Qed.
+
+
+Lemma step_needed_space prom0 prom1 mem0 mem1 cap0
+      loc from to msg kind
+      (spaces lefts: Loc.t -> Time.t -> Prop)
+      (PROMISE: Memory.promise prom0 mem0 loc from to msg prom1 mem1 kind)
+      (WRITENOTIN: forall ts (ITV: Interval.mem (from, to) ts), ~ spaces loc ts)
+      (WRITENOTTO: ~ lefts loc to)
+      (SOUND: Memory.le mem0 cap0)
+      (SPACES:
+         forall loc ts (COV: covered loc ts cap0),
+           <<COV: covered loc ts mem0>> \/ <<SPACE: spaces loc ts>>)
+      (UNATTACHABLE:
+         forall loc ts (COV: unattachable cap0 loc ts),
+           <<COV: unattachable mem0 loc ts>> \/ <<LEFT: lefts loc ts>>)
+      (MEM0: Memory.closed mem0)
+      (PROM0: Memory.le prom0 mem0)
+      (PROM1: Memory.le prom0 cap0)
+      (WF: kind <> Memory.op_kind_cancel)
+  :
+    exists cap1,
+      (<<STEP: Memory.promise prom0 cap0 loc from to msg prom1 cap1 kind>>) /\
+      (<<SOUND: Memory.le mem1 cap1>>) /\
+      (<<SPACES:
+         forall loc ts (COV: covered loc ts cap1),
+           <<COV: covered loc ts mem1>> \/ spaces loc ts>>) /\
+      (<<UNATTACHABLE:
+         forall loc ts (COV: unattachable cap1 loc ts),
+           <<COV: unattachable mem1 loc ts>> \/ lefts loc ts>>).
+Proof.
+  inv PROMISE.
+  { exploit add_succeed_wf; try apply MEM; eauto. i. des.
+    exploit (@Memory.add_exists cap0 loc from to msg); eauto.
+    { ii. exploit SPACES.
+      { econs; eauto. }
+      i. des.
+      { inv COV. eapply DISJOINT; eauto. }
+      { eapply WRITENOTIN; eauto. }
+    }
+    i. des. esplits.
+    { econs; eauto. i. exploit UNATTACHABLE.
+      { econs; eauto. eapply Memory.add_get0; eauto. }
+      i. des.
+      { inv COV. eapply ATTACH; eauto. }
+      { eapply WRITENOTTO; eauto. }
+    }
+    { ii. erewrite Memory.add_o in LHS; eauto.
+      erewrite (@Memory.add_o mem2 cap0); eauto. des_ifs.
+      eapply SOUND; eauto. }
+    { i. erewrite add_covered in COV; eauto.
+      erewrite (@add_covered mem1 mem0); eauto. des; eauto.
+      eapply SPACES in COV. des; auto. }
+    { i. erewrite add_unattachable in COV; eauto.
+      erewrite (@add_unattachable mem1 mem0); eauto. des_ifs; eauto.
+      ss. des; clarify. destruct p. eapply SOUND in Heq. clarify. }
+  }
+  { des. subst.
+    exploit (@Memory.split_exists_le prom0 cap0); eauto. i. des. esplits.
+    { econs; eauto. }
+    { ii. erewrite Memory.split_o in LHS; eauto.
+      erewrite (@Memory.split_o mem2 cap0); eauto. des_ifs.
+      eapply SOUND; eauto. }
+    { i. erewrite (@split_covered mem2 cap0) in COV; eauto.
+      erewrite (@split_covered mem1 mem0); eauto. }
+    { i. erewrite (@split_unattachable mem2 cap0) in COV; eauto.
+      erewrite (@split_unattachable mem1 mem0); eauto. }
+  }
+  { des. subst.
+    exploit (@Memory.lower_exists_le prom0 cap0); eauto. i. des. esplits.
+    { econs; eauto. }
+    { ii. erewrite Memory.lower_o in LHS; eauto.
+      erewrite (@Memory.lower_o mem2 cap0); eauto. des_ifs.
+      eapply SOUND; eauto. }
+    { i. erewrite (@lower_covered mem2 cap0) in COV; eauto.
+      erewrite (@lower_covered mem1 mem0); eauto. }
+    { i. erewrite (@lower_unattachable mem2 cap0) in COV; eauto.
+      erewrite (@lower_unattachable mem1 mem0); eauto. }
+  }
+  { ss. }
+Qed.
+
+
+
+
+Lemma step_lifting lang st0 st1 lc0 lc1 tm0 tm1 mem0 mem1 cap0 pf e
+      (spaces lefts: Loc.t -> Time.t -> Prop)
+      (STEP: Thread.step pf e (Thread.mk lang st0 lc0 tm0 mem0) (Thread.mk _ st1 lc1 tm1 mem1))
+      (WRITENOTIN: write_not_in spaces e)
+      (WRITENOTTO: write_not_to lefts e)
+      (SOUND: Memory.le mem0 cap0)
+      (SPACES:
+         forall loc ts (COV: covered loc ts cap0),
+           <<COV: covered loc ts mem0>> \/ <<SPACE: spaces loc ts>>)
+      (UNATTACHABLE:
+         forall loc ts (COV: unattachable cap0 loc ts),
+           <<COV: unattachable mem0 loc ts>> \/ <<LEFT: lefts loc ts>>)
+      (MEM0: Memory.closed mem0)
+      (* (MEM1: Memory.closed cap0) *)
+      (LOCAL0: Local.wf lc0 mem0)
+      (SC0: Memory.closed_timemap tm0 mem0)
+  :
+    exists cap1,
+      (<<STEP: Thread.step pf e (Thread.mk _ st0 lc0 tm0 cap0) (Thread.mk _ st1 lc1 tm1 cap1)>>) /\
+      (<<SOUND: Memory.le mem1 cap1>>) /\
+      (<<SPACES:
+         forall loc ts (COV: covered loc ts cap1),
+           <<COV: covered loc ts mem1>> \/ spaces loc ts>>) /\
+      (<<UNATTACHABLE:
+         forall loc ts (COV: unattachable cap1 loc ts),
+           <<COV: unattachable mem1 loc ts>> \/ lefts loc ts>>).
+Proof.
+  assert (LOCAL1: Local.wf lc0 cap0).
+  { eapply memory_concrete_le_local_wf; eauto.
+    etrans; eauto. eapply LOCAL0. }
+  assert (SC1: Memory.closed_timemap tm0 cap0).
+  { eapply memory_concrete_le_closed_timemap; eauto. }
+  inv STEP.
+  { inv STEP0. inv LOCAL. inv PROMISE.
+    { exploit add_succeed_wf; eauto. i. des.
+
+      Memory.promise
+      exploit Memory.add_exists_le
+
+      Memory.add
+
+
+
+
+         write_not_in
+
+                  ~ write_not_in aaa, ~ covered aaa mem0, ~ covered aa mem1
+                                                            ~
+
+      (SOUND: Memory.le mem0 cap0)
+      (U
+
+      Thread.mk
+
+
+
+
+           (ADJ: Memory.adjacent
+
+
+
+           Memory.adjacent
+
+
+
+Definition pf_consistent_strong_aux lang (e0:Thread.t lang): Prop :=
+  forall mem1
+         (CAP: Memory.cap e0.(Thread.memory) mem1),
+  exists tr_cancel tr e1 times,
+    (<<STEPS: Trace.steps (tr_cancel ++ tr) (Thread.mk _ e0.(Thread.state) e0.(Thread.local) TimeMap.bot mem1) e1>>) /\
+    (<<CANCELS: List.Forall (fun em => <<SAT: is_cancel (snd em)>>) tr_cancel>>) /\
+    (<<CANCELS: List.Forall (fun em => <<SAT: (fun e => ~ is_cancel e) (snd em)>>) tr_cancel>>) /\
+    (<<EVENTS: List.Forall (fun em => <<SAT: (promise_free /1\ no_sc /1\ (wf_time_evt (fun loc to => List.In to (times loc)))) (snd em)>> /\ <<TAU: ThreadEvent.get_machine_event (snd em) = MachineEvent.silent>>) tr >>) /\
+    (__guard__((exists st',
+                   (<<LOCAL: Local.failure_step e1.(Thread.local)>>) /\
+                   (<<FAILURE: Language.step lang ProgramEvent.failure (@Thread.state lang e1) st'>>)) \/
+               ((<<PROMISES: e1.(Thread.local).(Local.promises) = Memory.bot>>)))).
+
+Lemma pf_consistent_strong_pf_consistent_strong_aux lang (th: Thread.t lang)
+      (WF: Local.wf th.(Thread.local) th.(Thread.memory))
+      (MEM: Memory.closed th.(Thread.memory))
+      (CONSISTENT: pf_consistent_strong th)
+  :
+    pf_consistent_strong_aux th.
+Proof.
+  ii. exploit CONSISTENT; eauto. i. des.
+  hexploit (proj1 (@pred_steps_trace_steps (promise_free /1\ no_sc) _ (Thread.mk _ th.(Thread.state) th.(Thread.local) TimeMap.bot mem1) e1)).
+
+
+
+  eapply pred_step_rtc_mon with (Q:=(promise_free /1\ no_sc /1\ is_cancel)) in STEPS0; cycle 1.
+  { i. destruct x1; ss. destruct kind; ss. }
+  eapply pred_step_rtc_mon with (Q:=(promise_free /1\ no_sc /1\ (fun e => ~ is_cancel e))) in STEPS1; cycle 1.
+  { i. des; auto. }
+  hexploit (proj1 (@pred_steps_trace_steps (promise_free /1\ no_sc) _ (Thread.mk _ th.(Thread.state) th.(Thread.local) TimeMap.bot mem1) e1)).
+  { eauto.
+
+    etrans; eauto. } i. des.
+
+
+  hexploit (proj1 (@pred_steps_trace_steps (promise_free /1\ no_sc) _ (Thread.mk _ th.(Thread.state) th.(Thread.local) TimeMap.bot mem1) e2)).
+  { etrans; eauto. } i. des.
+  exploit trace_times_list_exists; eauto. i. des.
+  eexists tr, e2, times. esplits; eauto.
+  { eapply list_Forall_sum.
+    { eapply EVENTS. }
+    { eapply WFTIME. }
+    i. ss. des. splits; auto. }
+Qed.
+
+Definition certification_times (times : Loc.t -> list Time.t)
+           (f: Loc.t -> nat -> (Time.t -> Time.t -> Prop))
+           (max: TimeMap.t)
+           (maxmap: TimeMap.t)
+           (loc: Loc.t) (fts: Time.t): Prop :=
+  ((<<IN: List.In fts (times loc)>>) /\ (<<TS: Time.le fts (max loc)>>)) \/
+  (exists ts n,
+      (<<IN: List.In ts (times loc)>>) /\ (<<TS: Time.lt (max loc) ts>>)
+      /\ (<<MAX: Time.lt (maxmap loc) (incr_time_seq n)>>)
+      /\ (<<MAP: f loc n ts fts>>)).
+
+Lemma certification_times_well_ordered times f max maxmap tm
+      (MAP: forall loc n
+                   (TS: Time.lt (maxmap loc) (incr_time_seq n)),
+          cap_flex_map_loc
+            (max loc)
+            (tm loc)
+            (incr_time_seq n) (times loc) (f loc n))
+      (TM: forall loc, Time.lt (maxmap loc) (tm loc))
+      (MAXMAP: TimeMap.le max maxmap)
+  :
+    forall loc, well_ordered (certification_times times f max maxmap loc).
+Proof.
+  i. hexploit (@increasing_join_well_ordered
+                 incr_time_seq
+                 (fun n fts =>
+                    (exists ts,
+                        (<<IN: List.In ts (times loc)>>)
+                        /\ (<<TS: Time.lt (max loc) ts>>)
+                        /\ (<<MAX: Time.lt (maxmap loc) (incr_time_seq n)>>)
+                        /\ (<<MAP: f loc n ts fts>>)))).
+  { i. eapply incr_time_seq_lt; eauto. }
+  { eapply incr_time_seq_diverge. }
+  { i. des. exploit MAP; eauto. intros FLEXMAP.
+    eapply (FLEXMAP.(cap_flex_map_loc_bound)); try apply MAP0. auto. }
+  { i. destruct (classic (Time.lt (maxmap loc) (incr_time_seq n))).
+    { specialize (MAP _ _ H). eapply mapped_well_ordered.
+      { eapply MAP. }
+      { eapply (finite_well_ordered (times loc)). }
+      i. des. esplits; eauto.
+    }
+    { eapply sub_well_ordered.
+      { eapply empty_well_ordered. }
+      i. des; ss.
+    }
+  }
+  intros WO.
+  eapply sub_well_ordered.
+  { eapply join_well_ordered.
+    { eapply WO. }
+    { eapply (finite_well_ordered (times loc)). }
+  }
+  { i. unfold certification_times in *. des; eauto. left. esplits; eauto. }
+Qed.
+
+
+Definition pf_consistent_flex lang (e0:Thread.t lang)
+           (tr : Trace.t) (times : Loc.t -> list Time.t)
+           (f: Loc.t -> nat -> (Time.t -> Time.t -> Prop))
+  : Prop :=
+  forall max
+         (MAX: concrete_promise_max_timemap
+                 (e0.(Thread.memory))
+                 (e0.(Thread.local).(Local.promises))
+                 max),
+    (<<MAP: forall loc n
+                   (TS: Time.lt (Memory.max_ts loc e0.(Thread.memory)) (incr_time_seq n)),
+        cap_flex_map_loc
+          (max loc)
+          (Time.incr (Memory.max_ts loc e0.(Thread.memory)))
+          (incr_time_seq n) (times loc) (f loc n)>>) /\
+    (<<CONSISTENT: forall mem1 (tm: Loc.t -> nat)
+                          (TM: forall loc, Time.lt (Memory.max_ts loc e0.(Thread.memory)) (incr_time_seq (tm loc)))
+                          (CAP: cap_flex e0.(Thread.memory) mem1 (fun loc => incr_time_seq (tm loc))),
+        exists ftr e1,
+          (<<STEPS: Trace.steps ftr (Thread.mk _ e0.(Thread.state) e0.(Thread.local) TimeMap.bot mem1) e1>>) /\
+          (<<EVENTS: List.Forall (fun em => <<SAT: (promise_free
+                                                      /1\ no_sc
+                                                      /1\ wf_time_evt (fun loc => certification_times times f max (Memory.max_timemap e0.(Thread.memory)) loc)) (snd em)>> /\ <<TAU: ThreadEvent.get_machine_event (snd em) = MachineEvent.silent>>) ftr >>) /\
+          (<<TRACE: List.Forall2 (fun em fem => tevent_map (fun loc => f loc (tm loc)) (snd fem) (snd em)) tr ftr>>) /\
+          (__guard__((exists st',
+                         (<<LOCAL: Local.failure_step e1.(Thread.local)>>) /\
+                         (<<FAILURE: Language.step lang ProgramEvent.failure (@Thread.state lang e1) st'>>)) \/
+                     (<<PROMISES: e1.(Thread.local).(Local.promises) = Memory.bot>>)))>>).
+
+
+Lemma pf_consistent_strong_aux_pf_consistent_flex lang (th: Thread.t lang)
+      (WF: Local.wf th.(Thread.local) th.(Thread.memory))
+      (MEM: Memory.closed th.(Thread.memory))
+      (CONSISTENT: pf_consistent_strong_aux th)
+  :
+    exists tr times f, <<CONSISTENT: pf_consistent_flex th tr times f>>.
+Proof.
+  exploit Memory.cap_exists; eauto. i. des.
+  exploit CONSISTENT; eauto. i. des. exists tr, times.
+  hexploit (@concrete_promise_max_timemap_exists
+              (th.(Thread.memory))
+              (th.(Thread.local).(Local.promises))).
+  { eapply MEM. } intros [max MAX]. des.
+  hexploit (@choice
+              (Loc.t * nat)
+              (Time.t -> Time.t -> Prop)
+              (fun locn f =>
+                 let (loc, n) := locn in
+                 forall
+                   (TS: Time.lt (Memory.max_ts loc th.(Thread.memory)) (incr_time_seq n)),
+                   cap_flex_map_loc
+                     (max loc)
+                     (Time.incr (Memory.max_ts loc th.(Thread.memory)))
+                     (incr_time_seq n) (times loc) f)).
+  { intros [loc n].
+    destruct (classic (Time.lt (Memory.max_ts loc th.(Thread.memory)) (incr_time_seq n))).
+    { des. hexploit (@cap_flex_map_loc_exists
+                       (max loc)
+                       (Time.incr (Memory.max_ts loc (Thread.memory th)))
+                       (incr_time_seq n)).
+      { eapply TimeFacts.le_lt_lt.
+        { eapply concrete_promise_max_ts_max_ts; eauto. eapply WF. }
+        { eapply Time.incr_spec. }
+      }
+      { eapply TimeFacts.le_lt_lt.
+        { eapply concrete_promise_max_ts_max_ts; eauto. eapply WF. }
+        { auto. }
+      }
+      i. des. eauto. }
+    { exists bot2. i. exfalso. eapply H. auto. }
+  }
+  intros [f SPEC]. des. exists (fun loc ts => f (loc, ts)). ii.
+  assert (max0 = max).
+  { eapply concrete_promise_max_timemap_inj; eauto. } subst. econs.
+  { ii. specialize (SPEC (loc, n)). ss. eauto. }
+  ii. assert (MAP: cap_flex_map
+                     max
+                     (fun loc => Time.incr (Memory.max_ts loc (Thread.memory th)))
+                     (fun loc => incr_time_seq (tm loc))
+                     times (fun loc => f (loc, tm loc))).
+  { eapply cap_flex_map_locwise. i.
+    eapply (SPEC (loc, tm loc)). eauto. }
+
+  assert (IDENT: map_ident_concrete (fun loc => f (loc, tm loc)) th.(Thread.memory)).
+  { ii. inv CONCRETE. eapply MAX in GET. eapply MAP; eauto. }
+  destruct e1. ss.
+  hexploit trace_steps_map.
+  { eapply mapping_map_lt_map_le. eapply MAP. }
+  { eapply MAP. }
+  { eapply mapping_map_lt_map_eq. eapply MAP. }
+  { eapply wf_time_mapped_mappable.
+    { eapply List.Forall_impl; eauto. i. ss. des; eauto. }
+    { eapply cap_flex_map_complete; eauto. }
+  }
+  { eapply STEPS. }
+  { ss. }
+  { ss. }
+  { ss. }
+  { eapply Local.cap_wf; eauto. }
+  { instantiate (1:=mem1). instantiate (1:=th.(Thread.local)).
+    eapply cap_flex_wf; eauto. }
+  { eapply cap_flex_closed; eauto. }
+  { eapply Memory.cap_closed; eauto. }
+  { eapply Memory.closed_timemap_bot.
+    eapply cap_flex_closed in CAP0; auto. eapply CAP0. }
+  { eapply Memory.closed_timemap_bot.
+    eapply Memory.cap_closed in CAP; auto. eapply CAP. }
+  { econs.
+    { refl. }
+    { eapply map_ident_concrete_closed_tview; eauto. eapply WF. }
+    { eapply map_ident_concrete_promises; eauto.
+      { i. eapply MAP; eauto. }
+      { eapply MAP. }
+      { eapply WF. }
+    }
+  }
+  { exploit (@Memory.max_concrete_timemap_exists th.(Thread.memory)).
+    { eapply MEM. } i. des.
+    eapply concrete_messages_le_cap_flex_memory_map.
+    { refl. }
+    { eauto. }
+    { ii. eapply concrete_promise_max_ts_max_concrete_ts; eauto. }
+    { instantiate (1:=(fun loc => Time.incr (Memory.max_ts loc th.(Thread.memory)))).
+      i. eapply Time.incr_spec. }
+    { eapply TM. }
+    { eapply cap_cap_flex; eauto. }
+    { eauto. }
+    { eauto. }
+    { eauto. }
+    { eauto. }
+  }
+  { eapply mapping_map_lt_collapsable_unwritable. eapply MAP. }
+  { eapply timemap_bot_map. eapply MAP. }
+  { refl. } i. des.
+  exists ftr, (Thread.mk _ state flc1 fsc1 fmem1). splits; auto.
+  { eapply List.Forall_forall. i.
+    cut ((promise_free /1\ no_sc) (snd x) /\ ThreadEvent.get_machine_event (snd x) = MachineEvent.silent).
+    { i. des. splits; auto.
+      { eapply list_Forall2_in in H; eauto. des.
+        eapply List.Forall_forall in IN; eauto. ss. des.
+        eapply wf_time_evt_map in EVENT; eauto. eapply wf_time_evt_mon; try apply EVENT.
+        i. ss. des. destruct (Time.le_lt_dec ts (max x0)).
+        { left. assert (ts = x2).
+          { eapply mapping_map_lt_map_eq.
+            { eapply MAP. }
+            { ss. eapply MAP. eauto. }
+            { eauto. }
+          }
+          subst. splits; auto.
+        }
+        { right. esplits; eauto. }
+      }
+    }
+    eapply list_Forall2_in in H; eauto. des.
+    eapply List.Forall_forall in IN; eauto. ss. des.
+    destruct x, a. ss. inv EVENT; ss. inv KIND; ss.
+    splits; auto. inv MSG0; ss. inv MSG; ss. inv MAP1; ss.
+  }
+  { eapply list_Forall2_impl; eauto. i. ss. des. auto. }
+  { ss. unguard. des; eauto.
+    { left. esplits; eauto. eapply failure_step_map; eauto.
+      { eapply mapping_map_lt_map_le. eapply MAP. }
+      { eapply mapping_map_lt_map_eq. eapply MAP. }
+    }
+    { right. splits.
+      { inv LOCAL. erewrite PROMISES in *. eapply bot_promises_map; eauto. }
+    }
+  }
+Qed.
+
+
+Definition pf_consistent_super_strong_easy lang (e0:Thread.t lang)
+           (tr : Trace.t)
+           (times: Loc.t -> (Time.t -> Prop))
+  : Prop :=
+  forall cap (tm: Loc.t -> nat) max
+         (CAPTM: forall loc, Time.lt (Memory.max_ts loc e0.(Thread.memory)) (incr_time_seq (tm loc)))
+         (CAP: cap_flex e0.(Thread.memory) cap (fun loc => incr_time_seq (tm loc)))
+         (MAX: concrete_promise_max_timemap
+                 (e0.(Thread.memory))
+                 (e0.(Thread.local).(Local.promises))
+                 max),
+  exists ftr e1 f,
+    (<<STEPS: Trace.steps ftr (Thread.mk _ e0.(Thread.state) e0.(Thread.local) TimeMap.bot cap) e1>>) /\
+    (<<EVENTS: List.Forall (fun em => <<SAT: (promise_free
+                                                /1\ no_sc
+                                                /1\ wf_time_evt times) (snd em)>> /\ <<TAU: ThreadEvent.get_machine_event (snd em) = MachineEvent.silent>>) ftr >>) /\
+    (<<MAPLT: mapping_map_lt f>>) /\
+    (<<MAPIDENT: forall loc ts fts
+                        (TS: Time.le fts (max loc))
+                        (MAP: f loc ts fts),
+        ts = fts>>) /\
+    (<<BOUND: forall loc ts fts (TS: Time.lt (max loc) fts) (MAP: f loc ts fts),
+        Time.lt (max loc) ts /\ Time.le (incr_time_seq (tm loc)) fts>>) /\
+    (<<TRACE: List.Forall2 (fun em fem => tevent_map_weak f (snd fem) (snd em)) tr ftr>>) /\
+    (__guard__((exists st',
+                   (<<LOCAL: Local.failure_step e1.(Thread.local)>>) /\
+                   (<<FAILURE: Language.step lang ProgramEvent.failure (@Thread.state lang e1) st'>>)) \/
+               (<<PROMISES: e1.(Thread.local).(Local.promises) = Memory.bot>>))).
+
+
+Lemma pf_consistent_flex_super_strong_easy
+      lang (th: Thread.t lang) tr times f
+      (WF: Local.wf th.(Thread.local) th.(Thread.memory))
+      (MEM: Memory.closed th.(Thread.memory))
+      (CONSISTENT: pf_consistent_flex th tr times f)
+  :
+    exists certimes,
+      (<<WO: forall loc, well_ordered (certimes loc)>>) /\
+      (<<CONSISTENT: pf_consistent_super_strong_easy th tr certimes>>).
+Proof.
+  hexploit (@concrete_promise_max_timemap_exists
+              (th.(Thread.memory))
+              (th.(Thread.local).(Local.promises))).
+  { eapply MEM. } intros [max MAX]. specialize (CONSISTENT _ MAX). des.
+  exists (certification_times times f max (Memory.max_timemap th.(Thread.memory))). splits.
+  { eapply certification_times_well_ordered; eauto.
+    { i. eapply MAP. auto. }
+    { i. ss. eapply Time.incr_spec. }
+    { ii. eapply concrete_promise_max_ts_max_ts; eauto. eapply WF. }
+  }
+  ii. assert (max0 = max).
+  { eapply concrete_promise_max_timemap_inj; eauto. } subst.
+  hexploit CONSISTENT0; eauto. i. des.
+  assert (MAPALL: cap_flex_map
+                    max
+                    (fun loc => Time.incr (Memory.max_ts loc (Thread.memory th)))
+                    (fun loc => incr_time_seq (tm loc))
+                    times (fun loc => f loc (tm loc))).
+  { eapply cap_flex_map_locwise; eauto. }
+  eexists _, _, (fun loc => f loc (tm loc)). splits; eauto.
+  { eapply MAPALL. }
+  { i. eapply MAPALL in TS; eauto.
+    eapply mapping_map_lt_inj.
+    { eapply MAPALL; eauto. }
+    { ss. eauto. }
+    { eauto. }
+  }
+  { i. destruct (Time.le_lt_dec ts (max loc)).
+    { dup l. eapply MAPALL in l; eauto.
+      exploit mapping_map_lt_map_eq.
+      { eapply MAPALL. }
+      { eapply MAP0. }
+      { eapply l. }
+      i. subst. timetac.
+    }
+    { split; auto. eapply MAPALL.(cap_flex_map_bound) in l; eauto. }
+  }
+  { eapply list_Forall2_impl; eauto. i. eapply tevent_map_tevent_map_weak; eauto. }
+Qed.
+
+
+Definition pf_consistent_super_strong_aux lang (e0:Thread.t lang)
+           (tr : Trace.t)
+           (times: Loc.t -> (Time.t -> Prop))
+  : Prop :=
+  forall cap (tm: Loc.t -> nat) max
+         (CAPTM: forall loc, Time.lt (Memory.max_ts loc e0.(Thread.memory)) (incr_time_seq (tm loc)))
+         (CAP: cap_flex e0.(Thread.memory) cap (fun loc => incr_time_seq (tm loc)))
+         (MAX: concrete_promise_max_timemap
+                 (e0.(Thread.memory))
+                 (e0.(Thread.local).(Local.promises))
+                 max),
+  exists ftr e1 f,
+    (<<STEPS: Trace.steps ftr (Thread.mk _ e0.(Thread.state) e0.(Thread.local) TimeMap.bot cap) e1>>) /\
+    (<<EVENTS: List.Forall (fun em => <<SAT: (promise_free
+                                                /1\ no_sc
+                                                /1\ no_read_msgs (fun loc ts => ~ (covered loc ts e0.(Thread.local).(Local.promises) \/ concrete_promised e0.(Thread.memory) loc ts \/ Time.lt (incr_time_seq (tm loc)) ts))
+                                                /1\ write_not_in (fun loc ts => (<<TS: Time.le ts (incr_time_seq (tm loc))>>) /\ (<<PROM: ~ covered loc ts e0.(Thread.local).(Local.promises)>>))
+                                                /1\ wf_time_evt times) (snd em)>> /\ <<TAU: ThreadEvent.get_machine_event (snd em) = MachineEvent.silent>>) ftr >>) /\
+    (<<MAPLT: mapping_map_lt f>>) /\
+    (<<MAPIDENT: forall loc ts fts
+                        (TS: Time.le fts (max loc))
+                        (MAP: f loc ts fts),
+        ts = fts>>) /\
+    (<<BOUND: forall loc ts fts (TS: Time.lt (max loc) fts) (MAP: f loc ts fts),
+        Time.lt (max loc) ts /\ Time.le (incr_time_seq (tm loc)) fts>>) /\
+    (<<TRACE: List.Forall2 (fun em fem => tevent_map_weak f (snd fem) (snd em)) tr ftr>>) /\
+    (__guard__((exists st',
+                   (<<LOCAL: Local.failure_step e1.(Thread.local)>>) /\
+                   (<<FAILURE: Language.step lang ProgramEvent.failure (@Thread.state lang e1) st'>>)) \/
+               (<<PROMISES: e1.(Thread.local).(Local.promises) = Memory.bot>>))).
+
+Lemma pf_consistent_super_strong_easy_aux
+      lang (th: Thread.t lang) tr times
+      (WF: Local.wf th.(Thread.local) th.(Thread.memory))
+      (MEM: Memory.closed th.(Thread.memory))
+      (CONSISTENT: pf_consistent_super_strong_easy th tr times)
+  :
+    pf_consistent_super_strong_aux th tr times.
+Proof.
+  ii. exploit CONSISTENT; eauto. i. des. esplits; eauto.
+  assert (MLE: Memory.le (Local.promises (Thread.local th)) cap).
+  { etrans.
+    { eapply WF. }
+    { eapply CAP. }
+  }
+  exploit write_not_in_traced; eauto.
+  intros WRITENOTIN.
+  exploit no_read_unreadable_traced; eauto.
+  intros NOREAD. ss.
+  eapply list_Forall_sum.
+  { eapply list_Forall_sum.
+    { eapply WRITENOTIN. }
+    { eapply NOREAD. }
+    instantiate (1:=fun lce => (no_read_msgs (fun loc ts => ~ (covered loc ts th.(Thread.local).(Local.promises) \/ concrete_promised th.(Thread.memory) loc ts \/ Time.lt (incr_time_seq (tm loc)) ts))
+                                             /1\ write_not_in (fun loc ts => (<<TS: Time.le ts (incr_time_seq (tm loc))>>) /\ (<<PROM: ~ covered loc ts th.(Thread.local).(Local.promises)>>))) (snd lce)).
+    i. ss. splits.
+    { eapply no_read_msgs_mon; eauto. i.
+      eapply not_or_and in PR. des.
+      eapply not_or_and in PR0. des. econs.
+      { eapply unwritable_eq; eauto. econs; eauto.
+        eapply cap_flex_covered; eauto. ss. econs; eauto.
+        { ss. destruct (Time.bot_spec x2); auto. inv H.
+          exfalso. eapply PR0. econs. eapply MEM. }
+        { ss. destruct (Time.le_lt_dec x2 (incr_time_seq (tm x0))); ss. }
+      }
+      { i. eapply PR0.
+        eapply cap_flex_inv in GET; eauto. des; ss. econs; eauto. }
+    }
+    { eapply write_not_in_mon_bot; eauto. i. des.
+      eapply unwritable_eq; eauto. econs; eauto.
+      eapply cap_flex_covered; eauto. ss. }
+  }
+  { eapply EVENTS. }
+  { i. ss. des. splits; auto. }
+Qed.
+
+
+Definition pf_consistent_super_strong_aux2 lang (e0:Thread.t lang)
+           (tr : Trace.t)
+           (times: Loc.t -> (Time.t -> Prop))
+  : Prop :=
+  forall mem1 tm max
+         (FUTURE: Memory.future_weak e0.(Thread.memory) mem1)
+         (CLOSED: Memory.closed mem1)
+         (LOCAL: Local.wf e0.(Thread.local) mem1)
+         (MAX: concrete_promise_max_timemap
+                 (e0.(Thread.memory))
+                 (e0.(Thread.local).(Local.promises))
+                 max),
+  exists ftr e1 f,
+    (<<STEPS: Trace.steps ftr (Thread.mk _ e0.(Thread.state) e0.(Thread.local) TimeMap.bot mem1) e1>>) /\
+    (<<EVENTS: List.Forall (fun em => <<SAT: (promise_free
+                                                /1\ no_sc
+                                                /1\ no_read_msgs (fun loc ts => ~ (covered loc ts e0.(Thread.local).(Local.promises) \/ concrete_promised e0.(Thread.memory) loc ts \/ Time.lt (tm loc) ts))
+                                                /1\ write_not_in (fun loc ts => (<<TS: Time.le ts (tm loc)>>) /\ (<<PROM: ~ covered loc ts e0.(Thread.local).(Local.promises)>>))
+                                                /1\ wf_time_evt times) (snd em)>> /\ <<TAU: ThreadEvent.get_machine_event (snd em) = MachineEvent.silent>>) ftr >>) /\
+    (<<MAPLT: mapping_map_lt f>>) /\
+    (<<MAPIDENT: forall loc ts fts
+                     (TS: Time.le fts (max loc))
+                     (MAP: f loc ts fts),
+        ts = fts>>) /\
+    (<<BOUND: forall loc ts fts (TS: Time.lt (max loc) fts) (MAP: f loc ts fts),
+        Time.lt (max loc) ts /\ Time.le (tm loc) fts>>) /\
+    (<<TRACE: List.Forall2 (fun em fem => tevent_map_weak f (snd fem) (snd em)) tr ftr>>) /\
+    (__guard__((exists st',
+                   (<<LOCAL: Local.failure_step e1.(Thread.local)>>) /\
+                   (<<FAILURE: Language.step lang ProgramEvent.failure (@Thread.state lang e1) st'>>)) \/
+               ((<<PROMISES: e1.(Thread.local).(Local.promises) = Memory.bot>>)))).
+
+Lemma ident_map_compose_tevent_weak f te0 te1 te2
+      (MAP0: tevent_map_weak f te1 te0)
+      (MAP1: tevent_map_weak ident_map te2 te1)
+  :
+    tevent_map_weak f te2 te0.
+Proof.
+  inv MAP0; inv MAP1; econs.
+  { inv FROM0. auto. }
+  { inv TO0. auto. }
+  { inv TO0. eauto. }
+  { inv FROM0. eauto. }
+  { inv TO0. eauto. }
+  { inv FROM0. eauto. }
+  { inv TO0. eauto. }
+Qed.
+
+Lemma ident_map_compose_tevent_weak2 f te0 te1 te2
+      (MAP0: tevent_map_weak ident_map te1 te0)
+      (MAP1: tevent_map_weak f te2 te1)
+  :
+    tevent_map_weak f te2 te0.
+Proof.
+  inv MAP0; inv MAP1; econs.
+  { inv FROM. auto. }
+  { inv TO. auto. }
+  { inv TO. eauto. }
+  { inv FROM. eauto. }
+  { inv TO. eauto. }
+  { inv FROM. eauto. }
+  { inv TO. eauto. }
+Qed.
+
+
+Lemma pf_consistent_super_strong_aux_aux2
+      lang (th: Thread.t lang) tr times
+      (WF: Local.wf th.(Thread.local) th.(Thread.memory))
+      (MEM: Memory.closed th.(Thread.memory))
+      (CONSISTENT: pf_consistent_super_strong_aux th tr times)
+  :
+    pf_consistent_super_strong_aux2 th tr times.
+Proof.
+  ii.
+  assert (TM: exists (ftm: Loc.t -> nat),
+             forall loc,
+               (<<TM0: Time.lt (Memory.max_ts loc th.(Thread.memory)) (incr_time_seq (ftm loc))>>) /\
+               (<<TM1: Time.lt (Memory.max_ts loc mem1) (incr_time_seq (ftm loc))>>) /\
+               (<<TM2: Time.le (tm loc) (incr_time_seq (ftm loc))>>)).
+  { eapply (choice
+              (fun loc n =>
+                 (<<TM0: Time.lt (Memory.max_ts loc th.(Thread.memory)) (incr_time_seq n)>>) /\
+                 (<<TM1: Time.lt (Memory.max_ts loc mem1) (incr_time_seq n)>>) /\
+                 (<<TM2: Time.le (tm loc) (incr_time_seq n)>>))).
+    intros loc. hexploit (incr_time_seq_diverge
+                            (Time.join (Time.join
+                                          (Memory.max_ts loc th.(Thread.memory))
+                                          (Memory.max_ts loc mem1))
+                                       (tm loc))).
+    i. des. exists n. splits.
+    { eapply TimeFacts.le_lt_lt; eauto. etrans.
+      { eapply Time.join_l. }
+      eapply Time.join_l. }
+    { eapply TimeFacts.le_lt_lt; eauto. etrans.
+      { eapply Time.join_r. }
+      eapply Time.join_l. }
+    { left. eapply TimeFacts.le_lt_lt; eauto.
+      eapply Time.join_r. }
+  }
+  des.
+  hexploit (@cap_flex_exists th.(Thread.memory) (fun loc => incr_time_seq (ftm loc))); eauto.
+  { i. eapply TM. }
+  intros [cap CAP]. des.
+  exploit CONSISTENT; eauto.
+  { i. eapply TM. }
+  i. des.
+  hexploit (@cap_flex_future_memory_map th.(Thread.memory)); eauto.
+  { i. eapply TM. }
+  { i. left. eapply TM. }
+  intros MEMORY. destruct e1. ss.
+  hexploit trace_steps_map.
+  { eapply ident_map_le; eauto. }
+  { eapply ident_map_bot; eauto. }
+  { eapply ident_map_eq; eauto. }
+  { eapply List.Forall_forall. i. eapply ident_map_mappable_evt. }
+  { eapply STEPS. }
+  { ss. }
+  { ss. }
+  { ss. }
+  { eapply cap_flex_wf; eauto. }
+  { eapply LOCAL. }
+  { eauto. }
+  { eapply cap_flex_closed; eauto. i. eapply TM. }
+  { eapply Memory.closed_timemap_bot; eauto. eapply CLOSED. }
+  { eapply Memory.closed_timemap_bot; eauto.
+    eapply cap_flex_closed; eauto. i. eapply TM. }
+  { eapply ident_map_local. }
+  { eauto. }
+  { eapply mapping_map_lt_collapsable_unwritable. eapply ident_map_lt. }
+  { eapply ident_map_timemap. }
+  { refl. }
+  i. des. esplits; eauto.
+  eapply List.Forall_forall. i.
+  eapply list_Forall2_in in H; eauto. des.
+  eapply List.Forall_forall in IN; eauto. ss. des.
+  destruct a, x. ss. splits; auto.
+  { inv EVENT; ss. inv FROM. inv TO. inv KIND; ss.
+    inv MSG0; ss. inv MSG; ss. inv MAP0; ss. }
+  { inv EVENT; ss. }
+  { inv EVENT; ss.
+    { inv TO. ii. eapply SAT2. ii. eapply H. des; auto.
+      right. right. eapply TimeFacts.le_lt_lt; eauto. apply TM. }
+    { inv FROM. ii. eapply SAT2. ii. eapply H. des; auto.
+      right. right. eapply TimeFacts.le_lt_lt; eauto. apply TM. }
+  }
+  { inv EVENT; ss.
+    { inv TO. inv FROM. inv KIND; ss. ii. eapply SAT1; eauto.
+      des. split; auto. red. etrans; eauto. eapply TM. }
+    { inv TO. inv FROM. ii. eapply SAT1; eauto.
+      des. split; auto. red. etrans; eauto. eapply TM. }
+    { inv TO. inv FROM. ii. eapply SAT1; eauto.
+      des. split; auto. red. etrans; eauto. eapply TM. }
+  }
+  { inv EVENT; ss.
+    { inv FROM. inv TO. auto. }
+    { inv FROM. inv TO. auto. }
+    { inv FROM. inv TO. auto. }
+  }
+  { inv EVENT; ss. }
+  { ii. exploit BOUND; eauto. i. des. split; auto.
+    etrans; eauto. eapply TM. }
+  { eapply list_Forall2_compose; eauto. i. ss. des.
+    eapply ident_map_compose_tevent_weak; eauto.
+    eapply tevent_map_tevent_map_weak; eauto.
+  }
+  { ss. unguard. des.
+    { left. esplits; eauto. eapply failure_step_map; eauto.
+      { eapply ident_map_le. }
+      { eapply ident_map_eq. }
+    }
+    { right. inv LOCAL0. rewrite PROMISES in *.
+      eapply bot_promises_map; eauto. }
+  }
+Qed.
+
+
+Definition pf_consistent_super_strong lang (e0:Thread.t lang)
+           (tr : Trace.t)
+           (times: Loc.t -> (Time.t -> Prop))
+  : Prop :=
+  forall mem1 tm sc max
+         (FUTURE: Memory.future_weak e0.(Thread.memory) mem1)
+         (CLOSED: Memory.closed mem1)
+         (LOCAL: Local.wf e0.(Thread.local) mem1)
+         (MAX: concrete_promise_max_timemap
+                 (e0.(Thread.memory))
+                 (e0.(Thread.local).(Local.promises))
+                 max),
+  exists ftr e1 f,
+    (<<STEPS: Trace.steps ftr (Thread.mk _ e0.(Thread.state) e0.(Thread.local) sc mem1) e1>>) /\
+    (<<EVENTS: List.Forall (fun em => <<SAT: (promise_free
+                                                /1\ no_sc
+                                                /1\ no_read_msgs (fun loc ts => ~ (covered loc ts e0.(Thread.local).(Local.promises) \/ concrete_promised e0.(Thread.memory) loc ts \/ Time.lt (tm loc) ts))
+                                                /1\ write_not_in (fun loc ts => (<<TS: Time.le ts (tm loc)>>) /\ (<<PROM: ~ covered loc ts e0.(Thread.local).(Local.promises)>>))
+                                                /1\ wf_time_evt times) (snd em)>> /\ <<TAU: ThreadEvent.get_machine_event (snd em) = MachineEvent.silent>>) ftr >>) /\
+    (<<MAPLT: mapping_map_lt f>>) /\
+    (<<MAPIDENT: forall loc ts fts
+                        (TS: Time.le fts (max loc))
+                        (MAP: f loc ts fts),
+        ts = fts>>) /\
+    (<<BOUND: forall loc ts fts (TS: Time.lt (max loc) fts) (MAP: f loc ts fts),
+        Time.lt (max loc) ts /\ Time.le (tm loc) fts>>) /\
+    (<<TRACE: List.Forall2 (fun em fem => tevent_map_weak f (snd fem) (snd em)) tr ftr>>) /\
+    (<<GOOD: good_future tm mem1 e1.(Thread.memory)>>) /\
+    (<<SC: e1.(Thread.sc) = sc>>) /\
+    (<<PROMCONSISTENT: Local.promise_consistent e1.(Thread.local)>>) /\
+    (__guard__((exists st',
+                   (<<LOCAL: Local.failure_step e1.(Thread.local)>>) /\
+                   (<<FAILURE: Language.step lang ProgramEvent.failure (@Thread.state lang e1) st'>>)) \/
+               ((<<PROMISES: e1.(Thread.local).(Local.promises) = Memory.bot>>) /\
+                (<<WRITES: forall loc from to val released
+                                  (GET: Memory.get loc to e0.(Thread.local).(Local.promises) = Some (from, Message.concrete val released)),
+                    exists th e,
+                      (<<WRITING: promise_writing_event loc from to val released e>>) /\
+                      (<<IN: List.In (th, e) ftr>>)>>)))).
+
+Lemma pf_consistent_super_strong_aux2_super_strong
+      lang (th: Thread.t lang) tr times
+      (WF: Local.wf th.(Thread.local) th.(Thread.memory))
+      (MEM: Memory.closed th.(Thread.memory))
+      (CONSISTENT: pf_consistent_super_strong_aux2 th tr times)
+  :
+    pf_consistent_super_strong th tr times.
+Proof.
+  ii. set (tm0:=TimeMap.join tm (fun loc => Time.incr (Memory.max_ts loc mem1))).
+  assert (TM0: forall loc, Time.lt (Memory.max_ts loc mem1) (tm0 loc)).
+  { i. eapply TimeFacts.lt_le_lt.
+    { eapply Time.incr_spec. }
+    { eapply Time.join_r. }
+  }
+  assert (TM1: TimeMap.le tm tm0).
+  { eapply TimeMap.join_l. }
+  exploit (CONSISTENT mem1 tm0 max); eauto. i. des. destruct e1. ss.
+  dup STEPS. eapply no_sc_any_sc_traced in STEPS; eauto; cycle 1.
+  { eapply List.Forall_impl; eauto. i. ss. des. auto. } des.
+  esplits; eauto.
+  { eapply List.Forall_impl; eauto. i. ss. des. splits; auto.
+    { eapply no_read_msgs_mon; eauto. ii. eapply PR. des; auto.
+      right. right. eapply TimeFacts.le_lt_lt; eauto. }
+    { eapply write_not_in_mon; eauto. ii. des. split; auto.
+      red. etrans; eauto. }
+  }
+  { ii. exploit BOUND; eauto. i. des. splits; auto. etrans; eauto. }
+  { eapply good_future_mon with (tm1:=tm0); auto.
+    eapply write_not_in_good_future_traced in STEPS0; eauto.
+    { ss. eapply Memory.closed_timemap_bot; eauto. eapply CLOSED. }
+    { eapply List.Forall_impl; eauto. i. ss. des. splits; auto.
+      eapply write_not_in_mon; eauto. ii. des. split; auto.
+      ii. eapply PR0. eapply memory_le_covered; eauto. eapply LOCAL. }
+  }
+  { eapply no_sc_same_sc_traced in STEPS1; eauto.
+    eapply List.Forall_impl; eauto. i. ss. des. auto. }
+  { unguard. des.
+    { inv LOCAL0. ss. }
+    { ss. eapply Local.bot_promise_consistent; eauto. }
+  }
+  { ss. unguard. des; eauto. right. splits; auto.
+    i. eapply steps_promise_decrease_promise_writing_event in STEPS1; eauto.
+    des; eauto. ss. erewrite PROMISES in *. erewrite Memory.bot_get in *. ss. }
+Qed.
+
+
+Lemma pf_consistent_super_strong_not_easy lang (th: Thread.t lang)
+      tr times
+      (LOCAL: Local.wf th.(Thread.local) th.(Thread.memory))
+      (MEM: Memory.closed th.(Thread.memory))
+      (CONSISTENT: pf_consistent_super_strong_easy th tr times)
+  :
+    pf_consistent_super_strong th tr times.
+Proof.
+  eapply pf_consistent_super_strong_aux2_super_strong; eauto.
+  eapply pf_consistent_super_strong_aux_aux2; eauto.
+  eapply pf_consistent_super_strong_easy_aux; eauto.
+Qed.
+
+Lemma consistent_pf_consistent_super_strong lang (th: Thread.t lang)
+      (LOCAL: Local.wf th.(Thread.local) th.(Thread.memory))
+      (MEM: Memory.closed th.(Thread.memory))
+      (CONSISTENT: Thread.consistent th)
+  :
+    exists tr certimes,
+      (<<WO: forall loc, well_ordered (certimes loc)>>) /\
+      <<CONSISTENT: pf_consistent_super_strong th tr certimes>>.
+Proof.
+  eapply consistent_pf_consistent in CONSISTENT; eauto.
+  eapply pf_consistent_pf_consistent_strong in CONSISTENT; eauto.
+  eapply pf_consistent_strong_pf_consistent_strong_aux in CONSISTENT; eauto.
+  eapply pf_consistent_strong_aux_pf_consistent_flex in CONSISTENT; eauto. des.
+  eapply pf_consistent_flex_super_strong_easy in CONSISTENT0; eauto. des.
+  eapply pf_consistent_super_strong_not_easy in CONSISTENT; eauto.
+Qed.
+
+Lemma pf_consistent_super_strong_consistent lang (th: Thread.t lang)
+      (LOCAL: Local.wf th.(Thread.local) th.(Thread.memory))
+      (MEM: Memory.closed th.(Thread.memory))
+      tr certimes
+      (CONSISTENT: pf_consistent_super_strong th tr certimes)
+  :
+    Thread.consistent th.
+Proof.
+  hexploit (@concrete_promise_max_timemap_exists
+              (th.(Thread.memory))
+              (th.(Thread.local).(Local.promises))).
+  { eapply MEM. } intros [max MAX]. des.
+  ii. exploit (CONSISTENT mem1 sc1 sc1).
+  { eapply Memory.cap_future_weak; eauto. }
+  { eapply Memory.cap_closed; eauto. }
+  { eapply Local.cap_wf; eauto. }
+  { eauto. }
+  i. des.
+  eapply pred_steps_trace_steps2 in STEPS; cycle 1.
+  { instantiate (1:=fun _ => True). eapply List.Forall_impl; eauto.
+    i. ss. des. splits; auto. }
+  eapply thread_steps_pred_steps in STEPS.
+  unguard. des.
+  { destruct e1. ss. left. econs. esplits; eauto. }
+  { right. esplits; eauto. }
+Qed.
+
+Definition pf_consistent_super_strong_mon lang e0 tr certimes0 certimes1
+           (CONSISTENT: @pf_consistent_super_strong
+                          lang e0 tr certimes0)
+           (LE: certimes0 <2= certimes1)
+  :
+    pf_consistent_super_strong e0 tr certimes1.
+Proof.
+  ii. exploit CONSISTENT; eauto. i. des. esplits; eauto.
+  eapply List.Forall_impl; eauto. i. ss. des. splits; auto.
+  eapply wf_time_evt_mon; eauto.
+Qed.
+
+Lemma promises_bot_certify_nil times lang (th: Thread.t lang)
+      (PROMISES: th.(Thread.local).(Local.promises) = Memory.bot)
+  :
+    pf_consistent_super_strong th [] times.
+Proof.
+  ii. eexists [], _, bot3. esplits; eauto.
+  { ii. ss. }
+  { ii. ss. }
+  { ii. ss. }
+  { refl. }
+  { eapply Local.bot_promise_consistent; eauto. }
+  { right. ss. splits; auto. i.
+    rewrite PROMISES in *. erewrite Memory.bot_get in *. ss. }
+Qed.
+
+Lemma failure_certify_nil times lang (th: Thread.t lang) st'
+      (FAILURE: Language.step lang ProgramEvent.failure (@Thread.state lang th) st')
+      (LOCAL: Local.failure_step th.(Thread.local))
+  :
+    pf_consistent_super_strong th [] times.
+Proof.
+  ii. eexists [], _, bot3. esplits; eauto.
+  { ii. ss. }
+  { ii. ss. }
+  { ii. ss. }
+  { refl. }
+  { inv LOCAL. ss. }
+  { left. ss. esplits; eauto. }
+Qed.
+
+Lemma certify_nil_promises_bot_or_failure times lang (th: Thread.t lang)
+      (CONSISTENT: pf_consistent_super_strong th [] times)
+      (CLOSED: Memory.closed th.(Thread.memory))
+      (LOCAL: Local.wf (Thread.local th) (Thread.memory th))
+  :
+    (<<PROMISES: th.(Thread.local).(Local.promises) = Memory.bot>>) \/
+    exists st',
+      (<<FAILURE: Language.step lang ProgramEvent.failure (@Thread.state lang th) st'>>) /\
+      (<<LOCAL: Local.failure_step th.(Thread.local)>>).
+Proof.
+  exploit concrete_promise_max_timemap_exists.
+  { eapply CLOSED. } i. des.
+  exploit (CONSISTENT (Thread.memory th) TimeMap.bot (Thread.sc th) tm); eauto.
+  { refl. } i. des. inv TRACE. inv STEPS; ss.
+  unguard. des; eauto.
+Qed.
+
+
+Lemma good_future_future_future mem0 mem_good0 mem_good1 tm
+      (f0: Loc.t -> Time.t -> Time.t -> Prop)
+      (IDENT: forall loc to fto (MAP: f0 loc to fto), to = fto)
+      (MAPBOT: mapping_map_bot f0)
+      (GOOD: memory_map f0 mem0 mem_good0)
+      (FUTURE: Memory.future_weak mem_good0 mem_good1)
+      (CLOSED: Memory.closed mem0)
+      (TM0: forall loc, Time.lt (Memory.max_ts loc mem_good1) (tm loc))
+      (TM1: forall loc, Time.lt (Memory.max_ts loc mem0) (tm loc))
+  :
+    exists mem1,
+      (<<CAP: cap_flex mem0 mem1 tm>>) /\
+      (<<MAP: memory_map ident_map mem1 mem_good1>>).
+Proof.
+  exploit (@cap_flex_exists mem0 tm); eauto. intros [mem1 CAP].
+  exists mem1. splits; auto. econs.
+  { i. eapply cap_flex_inv in GET; eauto. des; auto.
+    apply GOOD in GET. des; auto. destruct fmsg as [val freleased|]; cycle 1.
+    { inv MSGLE. inv MSG. auto. }
+    eapply Memory.future_weak_get1 in GET; eauto. des.
+    dup MSG. dup MSGLE. dup MSG_LE.
+    inv MSG; inv MSGLE; inv MSG_LE; auto.
+    right. esplits; cycle 3.
+    { eauto. }
+    { eapply IDENT; eauto. }
+    { eapply message_map_incr; eauto. }
+    { econs; eauto. }
+  }
+  { i. left. exists (tm loc), Time.bot, (tm loc), Time.bot. splits; ss.
+    { eapply Time.bot_spec. }
+    { eapply Memory.max_ts_spec in GET. des. left.
+      eapply TimeFacts.le_lt_lt; eauto. }
+    { i. erewrite cap_flex_covered in ITV; eauto. }
+  }
+Qed.
+
+Lemma good_future_consistent times lang st lc_src lc_tgt sc_src sc_tgt mem_src mem_tgt tr
+      (f: Loc.t -> Time.t -> Time.t -> Prop)
+      (CONSISTENT: pf_consistent_super_strong
+                     (Thread.mk lang st lc_tgt sc_tgt mem_tgt)
+                     tr times)
+      (IDENT: forall loc to fto (MAP: f loc to fto), to = fto)
+      (MAPBOT: mapping_map_bot f)
+      (LOCALSRC: Local.wf lc_src mem_src)
+      (LOCALTGT: Local.wf lc_tgt mem_tgt)
+      (MEMSRC: Memory.closed mem_src)
+      (MEMTGT: Memory.closed mem_tgt)
+      (LOCAL: local_map f lc_tgt lc_src)
+      (MEM: memory_map f mem_tgt mem_src)
+      max_tgt
+      (MAXTGT: concrete_promise_max_timemap mem_tgt lc_tgt.(Local.promises) max_tgt)
+  :
+    exists tr_good f_good,
+      (<<MAPLT: mapping_map_lt f_good>>) /\
+      (<<MAPIDENT: forall loc ts fts
+                          (TS: Time.le fts (max_tgt loc))
+                          (MAP: f_good loc ts fts),
+          ts = fts>>) /\
+      (<<BOUND: forall loc ts fts (TS: Time.lt (max_tgt loc) fts) (MAP: f_good loc ts fts),
+          Time.lt (max_tgt loc) ts /\ Time.lt (Memory.max_ts loc mem_tgt) fts>>) /\
+      (<<TRACE: List.Forall2 (fun em fem => tevent_map_weak f_good (snd fem) (snd em)) tr tr_good>>) /\
+      (<<CONSISTENT:
+         pf_consistent_super_strong (Thread.mk lang st lc_src sc_src mem_src) tr_good times>>)
+.
+Proof.
+  hexploit (CONSISTENT mem_tgt (fun loc => Time.incr (Time.join (Memory.max_ts loc mem_tgt) (Memory.max_ts loc mem_src))) sc_tgt); eauto.
+  { refl. } ss.
+  intros [tr_good [e1_good [f_good [STEPSGOOD [EVENTSGOOD [MAPLTGOOD [IDENTGOOD [BOUNDGOOD [TRACEGOOD [GOODFUTURE [SCGOOD GOODEND]]]]]]]]]]]. des.
+  exists tr_good, f_good. splits; auto.
+  { i. eapply BOUNDGOOD in MAP; eauto. des. splits; eauto.
+    eapply TimeFacts.lt_le_lt; eauto. eapply TimeFacts.le_lt_lt.
+    { eapply Time.join_l. }
+    { eapply Time.incr_spec. }
+  }
+  eapply pf_consistent_super_strong_not_easy; eauto. ii. ss.
+  assert (MAXMAP: TimeMap.le max_tgt max).
+  { eapply memory_ident_map_concrete_promise_max_timemap; eauto.
+    eapply LOCAL. }
+
+  set (tm0 := TimeMap.join (fun loc => incr_time_seq (tm loc))
+                           (fun loc => Time.incr
+                                         (Time.join
+                                            (max loc)
+                                            (Time.join
+                                               (Memory.max_ts loc cap)
+                                               (Memory.max_ts loc mem_tgt))))).
+  assert (TM0: forall loc, Time.lt (Memory.max_ts loc cap) (tm0 loc)).
+  { i. unfold tm0. eapply TimeFacts.le_lt_lt.
+    { eapply Time.join_l. } eapply TimeFacts.le_lt_lt.
+    { eapply Time.join_r. } eapply TimeFacts.lt_le_lt.
+    { eapply Time.incr_spec. }
+    { eapply Time.join_r. }
+  }
+  assert (TM1: forall loc, Time.lt (Memory.max_ts loc mem_tgt) (tm0 loc)).
+  { i. unfold tm0. eapply TimeFacts.le_lt_lt.
+    { eapply Time.join_r. } eapply TimeFacts.le_lt_lt.
+    { eapply Time.join_r. } eapply TimeFacts.lt_le_lt.
+    { eapply Time.incr_spec. }
+    { eapply Time.join_r. }
+  }
+  assert (TM2: TimeMap.le (fun loc => incr_time_seq (tm loc)) tm0).
+  { eapply TimeMap.join_l. }
+  assert (TM3: forall loc, Time.lt (max loc) (tm0 loc)).
+  { i. unfold tm0. eapply TimeFacts.le_lt_lt.
+    { eapply Time.join_l. } eapply TimeFacts.lt_le_lt.
+    { eapply Time.incr_spec. }
+    { eapply Time.join_r. }
+  }
+  exploit (@good_future_future_future mem_tgt mem_src cap); eauto.
+  { eapply cap_flex_future_weak; eauto. }
+  i. des.
+
+  exploit (CONSISTENT mem1 tm0 TimeMap.bot); eauto.
+  { ss. eapply cap_flex_future_weak; eauto. }
+  { eapply cap_flex_closed; eauto. }
+  { ss. eapply cap_flex_wf; eauto. }
+  ss. i. des. destruct e1. ss.
+  hexploit trace_steps_map.
+  { eapply ident_map_le; eauto. }
+  { eapply ident_map_bot; eauto. }
+  { eapply ident_map_eq; eauto. }
+  { eapply List.Forall_forall. i. eapply ident_map_mappable_evt. }
+  { eauto. }
+  { ss. }
+  { ss. }
+  { ss. }
+  { eapply cap_flex_wf; eauto. }
+  { eapply cap_flex_wf; try apply CAP; eauto. }
+  { eapply cap_flex_closed; eauto. }
+  { eapply cap_flex_closed; eauto. }
+  { eapply Memory.closed_timemap_bot.
+    eapply cap_flex_closed; eauto. }
+  { eapply Memory.closed_timemap_bot.
+    eapply cap_flex_closed; eauto. }
+  { eapply local_map_incr; eauto. eapply ident_map_lt; eauto. }
+  { eauto. }
+  { eapply mapping_map_lt_collapsable_unwritable; eauto. eapply ident_map_lt. }
+  { eapply ident_map_timemap. }
+  { refl. }
+  i. des.
+  eexists ftr0, _, (fun loc ts0 ts2 => exists ts1, <<TS0: f_good loc ts1 ts0>> /\ <<TS1: f0 loc ts1 ts2>>).
+  esplits; eauto; ss.
+  { eapply List.Forall_forall. i. eapply list_Forall2_in in H; eauto. des.
+    eapply List.Forall_forall in IN; eauto. ss. des. destruct a, x. ss.
+    inv EVENT; splits; ss.
+    { inv KIND; ss. inv MSG0; ss. inv MSG; ss. inv MAP1; ss. }
+    { inv FROM. inv TO. auto. }
+    { inv FROM. inv TO. auto. }
+    { inv FROM. inv TO. auto. }
+  }
+  { ii. des. erewrite <- (MAPLTGOOD loc ts0 ts1 t0 t1); eauto. }
+  { ii. des.
+    destruct (Time.le_lt_dec fts (max_tgt loc)).
+    { dup l. eapply MAPIDENT in l; cycle 1; eauto. subst.
+      destruct (Time.le_lt_dec ts (max_tgt loc)).
+      { dup l. eapply IDENTGOOD in l; eauto. }
+      { dup l. eapply BOUNDGOOD in l; eauto. des. timetac. }
+    }
+    { dup l. eapply BOUND in l; cycle 1; eauto. des.
+      exfalso. eapply Time.lt_strorder. eapply TimeFacts.le_lt_lt.
+      { eapply l1. } eapply TimeFacts.le_lt_lt.
+      { eapply TS. }
+      auto.
+    }
+  }
+  { ii. des.
+    destruct (Time.le_lt_dec fts (max_tgt loc)).
+    { dup l. eapply MAPIDENT in l; cycle 1; eauto. subst.
+      exfalso. eapply Time.lt_strorder. eapply TimeFacts.le_lt_lt.
+      { eapply l0. } eapply TimeFacts.le_lt_lt.
+      { eapply MAXMAP. }
+      auto.
+    }
+    { dup l. eapply BOUND in l; cycle 1; eauto. des. splits; eauto.
+      destruct (Time.le_lt_dec ts (max_tgt loc)).
+      { dup l2. eapply IDENTGOOD in l2; eauto. subst. timetac. }
+      { dup l2. eapply BOUNDGOOD in l2; eauto. des.
+        eapply TimeFacts.le_lt_lt.
+        { eapply concrete_promise_max_ts_max_ts; eauto. eapply LOCALSRC. } eapply TimeFacts.le_lt_lt.
+        { eapply Time.join_r. } eapply TimeFacts.lt_le_lt.
+        { eapply Time.incr_spec. }
+        eauto.
+      }
+    }
+  }
+  { dup TRACEGOOD. dup TRACE. dup TRACE0.
+    eapply list_Forall2_compose.
+    { eapply list_Forall2_rev. eapply TRACEGOOD. }
+    { eapply list_Forall2_compose.
+      { eapply TRACE. }
+      { eapply TRACE0. }
+      simpl. instantiate (1:=fun the fthe => tevent_map_weak f0 (snd fthe) (snd the)).
+      i. ss. des. eapply tevent_map_tevent_map_weak in EVENT.
+      eapply tevent_map_weak_compose; eauto.
+      i. inv MAP1. auto.
+    }
+    i. ss. eapply tevent_map_weak_rev in SAT0.
+    { instantiate (1:=fun loc ts fts => f_good loc fts ts) in SAT0.
+      eapply tevent_map_weak_compose; eauto.
+      i. ss. eauto. }
+    { i. ss. }
+  }
+  { clear GOODEND0. unguard. des.
+    { left. esplits; eauto. eapply failure_step_map; eauto.
+      { eapply ident_map_le. }
+      { eapply ident_map_eq. }
+    }
+    { inv LOCAL0. right. rewrite PROMISES in *.
+      eapply bot_promises_map in PROMISES0; eauto. }
+  }
+Qed.
