src/prop/PreReserve.v
@@ -1,0 +1,1128 @@
+Require Import Omega.
+Require Import Bool.
+Require Import RelationClasses.
+
+From sflib Require Import sflib.
+From Paco Require Import paco.
+
+From PromisingLib Require Import Axioms.
+From PromisingLib Require Import Basic.
+From PromisingLib Require Import DataStructure.
+From PromisingLib Require Import DenseOrder.
+From PromisingLib Require Import Language.
+From PromisingLib Require Import Loc.
+
+Require Import Event.
+Require Import Time.
+Require Import View.
+Require Import Cell.
+Require Import Memory.
+Require Import TView.
+Require Import Local.
+Require Import Thread.
+Require Import Pred.
+Require Import Trace.
+
+Require Import MemoryMerge.
+Require Import ReorderCancel.
+Require Import MemoryProps.
+Require Import OrderedTimes.
+Require Import Cover.
+
+Set Implicit Arguments.
+
+
+
+Lemma promise_not_cancel_covered_increase prom0 prom1 mem0 mem1
+      loc from to msg kind
+      (PROMISE: Memory.promise prom0 mem0 loc from to msg prom1 mem1 kind)
+      (NOTCANCEL: kind <> Memory.op_kind_cancel)
+      loc0 ts0
+      (COVERED: covered loc0 ts0 mem0)
+  :
+    covered loc0 ts0 mem1.
+Proof.
+  inv PROMISE.
+  { erewrite (@add_covered mem1 mem0); eauto. }
+  { erewrite (@split_covered mem1 mem0); eauto. }
+  { erewrite (@lower_covered mem1 mem0); eauto. }
+  { ss. }
+Qed.
+
+Lemma step_not_cancel_covered_increase lang (th0 th1: Thread.t lang) pf e
+      (STEP: Thread.step pf e th0 th1)
+      (NOTCANCEL: ~ is_cancel e)
+      loc0 ts0
+      (COVERED: covered loc0 ts0 th0.(Thread.memory))
+  :
+    covered loc0 ts0 th1.(Thread.memory).
+Proof.
+  inv STEP.
+  { inv STEP0. inv LOCAL. ss.
+    eapply promise_not_cancel_covered_increase; eauto. destruct kind; ss.
+  }
+  { inv STEP0. inv LOCAL; auto.
+    { inv LOCAL0. inv WRITE. eapply promise_not_cancel_covered_increase; eauto.
+      destruct kind; ss. inv PROMISE; ss. }
+    { inv LOCAL2. inv WRITE. eapply promise_not_cancel_covered_increase; eauto.
+      destruct kind; ss. inv PROMISE; ss. }
+  }
+Qed.
+
+Lemma traced_steps_not_cancel_covered_increase lang (th0 th1: Thread.t lang) tr
+      (STEPS: Trace.steps tr th0 th1)
+      (EVENTS: List.Forall (fun em => <<SAT: (fun e => ~ is_cancel e) (snd em)>>) tr)
+      loc0 ts0
+      (COVERED: covered loc0 ts0 th0.(Thread.memory))
+  :
+    covered loc0 ts0 th1.(Thread.memory).
+Proof.
+  ginduction STEPS; auto. i. clarify. inv EVENTS.
+  eapply step_not_cancel_covered_increase in STEP; eauto.
+Qed.
+
+
+
+Section UNATTACHABLE.
+
+  Inductive unattachable (mem: Memory.t) (loc: Loc.t) (ts: Time.t): Prop :=
+  | unattachable_intro
+      from to msg
+      (MSG: Memory.get loc to mem = Some (from, msg))
+      (FROM: Time.le from ts)
+      (TO: Time.lt ts to)
+  .
+
+  Lemma lower_unattachable mem1 mem0 loc from to msg1 msg2
+        (LOWER: Memory.lower mem0 loc from to msg1 msg2 mem1)
+    :
+      unattachable mem1 = unattachable mem0.
+  Proof.
+    extensionality loc0. extensionality ts0.
+    exploit Memory.lower_get0; eauto. i. des.
+    apply Coq.Logic.PropExtensionality.propositional_extensionality. split; i.
+    { inv H. erewrite Memory.lower_o in MSG; eauto. des_ifs.
+      { ss. des; clarify. econs; eauto. }
+      { econs; eauto. }
+    }
+    { inv H. eapply Memory.lower_get1 in MSG; eauto. des. econs; eauto. }
+  Qed.
+
+  Lemma split_unattachable mem1 mem0 loc ts1 ts2 ts3 msg2 msg3
+        (SPLIT: Memory.split mem0 loc ts1 ts2 ts3 msg2 msg3 mem1)
+    :
+      unattachable mem1 = unattachable mem0.
+  Proof.
+    extensionality loc0. extensionality ts0.
+    exploit split_succeed_wf; eauto. i. des.
+    exploit Memory.split_get0; eauto. i. des.
+    apply Coq.Logic.PropExtensionality.propositional_extensionality. split; i.
+    { inv H. erewrite Memory.split_o in MSG; eauto. des_ifs.
+      { ss. des; clarify. econs; eauto. }
+      { ss. des; clarify. econs; eauto. etrans; eauto. left. auto. }
+      { econs; eauto. }
+    }
+    { inv H. generalize (Memory.split_o loc0 to SPLIT). intros MSG0. des_ifs.
+      { ss. des; clarify. }
+      { ss. des; clarify.
+        destruct (Time.le_lt_dec ts2 ts0).
+        { econs; try apply MSG0; eauto. }
+        { econs; try apply GET1; eauto. }
+      }
+      { erewrite MSG in *. clarify. econs; eauto. }
+    }
+  Qed.
+
+  Lemma add_unattachable mem1 mem0 loc from to msg
+        (ADD: Memory.add mem0 loc from to msg mem1)
+    :
+      unattachable mem1 =
+      (fun loc0 ts0 =>
+         unattachable mem0 loc0 ts0 \/ (loc0 = loc /\ Time.le from ts0 /\ Time.lt ts0 to)).
+  Proof.
+    extensionality loc0. extensionality ts0.
+    exploit add_succeed_wf; eauto. i.  des.
+    exploit Memory.add_get0; eauto. i. des.
+    apply Coq.Logic.PropExtensionality.propositional_extensionality. split; i.
+    { inv H. erewrite Memory.add_o in MSG; eauto. des_ifs.
+      { ss. des; clarify. right. splits; auto. }
+      { left. econs; eauto. }
+    }
+    { des; subst.
+      { inv H. econs; eauto. eapply Memory.add_get1; eauto. }
+      { econs; eauto. }
+    }
+  Qed.
+
+End UNATTACHABLE.
+
+
+
+Section LIFT.
+
+  Lemma memory_remove_le_preserve mem0 mem0' mem1 mem1' loc from to msg
+        (REMOVE0: Memory.remove mem0 loc from to msg mem0')
+        (REMOVE1: Memory.remove mem1 loc from to msg mem1')
+        (MLE: Memory.le mem0 mem1)
+  :
+    Memory.le mem0' mem1'.
+  Proof.
+    ii. erewrite Memory.remove_o; eauto.
+    erewrite (@Memory.remove_o mem0' mem0) in LHS; eauto. des_ifs.
+    eapply MLE; eauto.
+  Qed.
+
+  Lemma memory_add_le_preserve mem0 mem0' mem1 mem1' loc from to msg
+        (ADD0: Memory.add mem0 loc from to msg mem0')
+        (ADD1: Memory.add mem1 loc from to msg mem1')
+        (MLE: Memory.le mem0 mem1)
+    :
+      Memory.le mem0' mem1'.
+  Proof.
+    ii. erewrite Memory.add_o; eauto.
+    erewrite (@Memory.add_o mem0' mem0) in LHS; eauto. des_ifs.
+    eapply MLE; eauto.
+  Qed.
+
+  Lemma memory_split_le_preserve mem0 mem0' mem1 mem1' loc ts1 ts2 ts3 msg2 msg3
+        (SPLIT0: Memory.split mem0 loc ts1 ts2 ts3 msg2 msg3 mem0')
+        (SPLIT1: Memory.split mem1 loc ts1 ts2 ts3 msg2 msg3 mem1')
+        (MLE: Memory.le mem0 mem1)
+    :
+      Memory.le mem0' mem1'.
+  Proof.
+    ii. erewrite Memory.split_o; eauto.
+    erewrite (@Memory.split_o mem0' mem0) in LHS; eauto. des_ifs.
+    eapply MLE; eauto.
+  Qed.
+
+  Lemma memory_lower_le_preserve mem0 mem0' mem1 mem1' loc from to msg1 msg2
+        (LOWER0: Memory.lower mem0 loc from to msg1 msg2 mem0')
+        (LOWER1: Memory.lower mem1 loc from to msg1 msg2 mem1')
+        (MLE: Memory.le mem0 mem1)
+    :
+      Memory.le mem0' mem1'.
+  Proof.
+    ii. erewrite Memory.lower_o; eauto.
+    erewrite (@Memory.lower_o mem0' mem0) in LHS; eauto. des_ifs.
+    eapply MLE; eauto.
+  Qed.
+
+  Lemma step_lifting_promise prom0 prom1 mem0 mem1 cap0
+        loc from to msg kind
+        (spaces lefts: Loc.t -> Time.t -> Prop)
+        (PROMISE: Memory.promise prom0 mem0 loc from to msg prom1 mem1 kind)
+        (WRITENOTIN: forall ts (ITV: Interval.mem (from, to) ts), ~ spaces loc ts)
+        (WRITENOTTO: ~ lefts loc to)
+        (SOUND: Memory.le mem0 cap0)
+        (SPACES:
+           forall loc ts (COV: covered loc ts cap0),
+             <<COV: covered loc ts mem0>> \/ <<SPACE: spaces loc ts>>)
+        (LEFTS:
+           forall loc ts (UNATTACHABLE: unattachable cap0 loc ts),
+             <<COV: unattachable mem0 loc ts>> \/ <<LEFT: lefts loc ts>>)
+        (MEM0: Memory.closed mem0)
+        (PROM0: Memory.le prom0 mem0)
+        (PROM1: Memory.le prom0 cap0)
+        (NOTCANCEL: kind <> Memory.op_kind_cancel)
+    :
+      exists cap1,
+        (<<STEP: Memory.promise prom0 cap0 loc from to msg prom1 cap1 kind>>) /\
+        (<<SOUND: Memory.le mem1 cap1>>) /\
+        (<<SPACES:
+           forall loc ts (COV: covered loc ts cap1),
+             <<COV: covered loc ts mem1>> \/ spaces loc ts>>) /\
+        (<<LEFTS:
+           forall loc ts (UNATTACHABLE: unattachable cap1 loc ts),
+             <<COV: unattachable mem1 loc ts>> \/ lefts loc ts>>).
+  Proof.
+    inv PROMISE.
+    { exploit add_succeed_wf; try apply MEM; eauto. i. des.
+      exploit (@Memory.add_exists cap0 loc from to msg); eauto.
+      { ii. exploit SPACES.
+        { econs; eauto. }
+        i. des.
+        { inv COV. eapply DISJOINT; eauto. }
+        { eapply WRITENOTIN; eauto. }
+      }
+      i. des. esplits.
+      { econs; eauto. i. subst. exploit LEFTS.
+        { econs; eauto.
+          { refl. }
+          { apply memory_get_ts_strong in GET. des; auto.
+            subst. eapply TimeFacts.le_lt_lt; eauto. eapply Time.bot_spec. }
+        }
+        i. des; ss.
+        { inv COV. destruct FROM.
+          { eapply DISJOINT; eauto.
+            { instantiate (1:=to). econs; ss. refl. }
+            { econs; ss. left. eauto. }
+          }
+          { inv H. eapply ATTACH; eauto. }
+        }
+      }
+      { eapply memory_add_le_preserve; eauto. }
+      { i. erewrite add_covered in COV; eauto.
+        erewrite (@add_covered mem1 mem0); eauto. des; eauto.
+        eapply SPACES in COV. des; auto. }
+      { i. erewrite add_unattachable in UNATTACHABLE; eauto.
+        erewrite (@add_unattachable mem1 mem0); eauto. des; auto.
+        eapply LEFTS in UNATTACHABLE. des; auto. }
+    }
+    { des. subst.
+      exploit (@Memory.split_exists_le prom0 cap0); eauto. i. des. esplits.
+      { econs; eauto. }
+      { ii. erewrite Memory.split_o in LHS; eauto.
+        erewrite (@Memory.split_o mem2 cap0); eauto. des_ifs.
+        eapply SOUND; eauto. }
+      { i. erewrite (@split_covered mem2 cap0) in COV; eauto.
+        erewrite (@split_covered mem1 mem0); eauto. }
+      { i. erewrite (@split_unattachable mem2 cap0) in UNATTACHABLE; eauto.
+        erewrite (@split_unattachable mem1 mem0); eauto. }
+    }
+    { des. subst.
+      exploit (@Memory.lower_exists_le prom0 cap0); eauto. i. des. esplits.
+      { econs; eauto. }
+      { ii. erewrite Memory.lower_o in LHS; eauto.
+        erewrite (@Memory.lower_o mem2 cap0); eauto. des_ifs.
+        eapply SOUND; eauto. }
+      { i. erewrite (@lower_covered mem2 cap0) in COV; eauto.
+        erewrite (@lower_covered mem1 mem0); eauto. }
+      { i. erewrite (@lower_unattachable mem2 cap0) in UNATTACHABLE; eauto.
+        erewrite (@lower_unattachable mem1 mem0); eauto. }
+    }
+    { ss. }
+  Qed.
+
+  Lemma step_lifting lang st0 st1 lc0 lc1 sc0 sc1 mem0 mem1 cap0 pf e
+        (spaces lefts: Loc.t -> Time.t -> Prop)
+        (STEP: Thread.step pf e (Thread.mk lang st0 lc0 sc0 mem0) (Thread.mk _ st1 lc1 sc1 mem1))
+        (WRITENOTIN: write_not_in spaces e)
+        (WRITENOTTO: write_not_to lefts e)
+        (NOTCANCEL: ~ is_cancel e)
+        (SOUND: Memory.le mem0 cap0)
+        (SPACES:
+           forall loc ts (COV: covered loc ts cap0),
+             <<COV: covered loc ts mem0>> \/ <<SPACE: spaces loc ts>>)
+        (LEFTS:
+           forall loc ts (UNATACHABLE: unattachable cap0 loc ts),
+             <<COV: unattachable mem0 loc ts>> \/ <<LEFT: lefts loc ts>>)
+       (MEM0: Memory.closed mem0)
+        (LOCAL0: Local.wf lc0 mem0)
+        (SC0: Memory.closed_timemap sc0 mem0)
+    :
+      exists cap1,
+        (<<STEP: Thread.step pf e (Thread.mk _ st0 lc0 sc0 cap0) (Thread.mk _ st1 lc1 sc1 cap1)>>) /\
+        (<<SOUND: Memory.le mem1 cap1>>) /\
+        (<<SPACES:
+           forall loc ts (COV: covered loc ts cap1),
+             <<COV: covered loc ts mem1>> \/ spaces loc ts>>) /\
+        (<<UNATTACHABLE:
+           forall loc ts (COV: unattachable cap1 loc ts),
+             <<COV: unattachable mem1 loc ts>> \/ lefts loc ts>>).
+
+  Proof.
+    inv STEP.
+    { inv STEP0. inv LOCAL. ss.
+      destruct (Memory.op_kind_is_cancel kind) eqn:KIND; ss.
+      { destruct kind; ss. }
+      exploit step_lifting_promise; eauto.
+      { eapply LOCAL0. }
+      { transitivity mem0; eauto. eapply LOCAL0. }
+      { destruct kind; ss. }
+      i. des. esplits; eauto. econs. econs.
+      { econs; eauto. eapply memory_concrete_le_closed_msg; eauto. }
+      { ss. destruct kind; ss. }
+    }
+    { inv STEP0. inv LOCAL.
+      { esplits; eauto. }
+      { inv LOCAL1. eapply SOUND in GET. esplits; eauto. }
+      { inv LOCAL1. inv WRITE. exploit step_lifting_promise; eauto.
+        { eapply LOCAL0. }
+        { transitivity mem0; eauto. eapply LOCAL0. }
+        { destruct kind; ss. inv PROMISE; ss. }
+        i. des. esplits; eauto. econs 2; eauto.
+      }
+      { inv LOCAL1. eapply SOUND in GET. inv LOCAL2. inv WRITE.
+        exploit step_lifting_promise; eauto.
+        { eapply LOCAL0. }
+        { transitivity mem0; eauto. eapply LOCAL0. }
+        { destruct kind; ss. inv PROMISE; ss. }
+        i. des. esplits; eauto. econs 2; eauto. econs; eauto. }
+      { esplits; eauto. }
+      { esplits; eauto. }
+      { esplits; eauto. }
+    }
+  Qed.
+
+  Lemma traced_step_lifting lang st0 st1 lc0 lc1 sc0 sc1 mem0 mem1 cap0 tr
+        (spaces lefts: Loc.t -> Time.t -> Prop)
+        (STEPS: Trace.steps tr (Thread.mk lang st0 lc0 sc0 mem0) (Thread.mk _ st1 lc1 sc1 mem1))
+        (EVENTS: List.Forall (fun em => <<SAT: (write_not_in spaces /1\ write_not_to lefts /1\ (fun e => ~ is_cancel e)) (snd em)>>) tr)
+        (SOUND: Memory.le mem0 cap0)
+        (SPACES:
+           forall loc ts (COV: covered loc ts cap0),
+             <<COV: covered loc ts mem0>> \/ <<SPACE: spaces loc ts>>)
+        (LEFTS:
+           forall loc ts (UNATACHABLE: unattachable cap0 loc ts),
+             <<COV: unattachable mem0 loc ts>> \/ <<LEFT: lefts loc ts>>)
+        (MEM0: Memory.closed mem0)
+        (LOCAL0: Local.wf lc0 mem0)
+        (SC0: Memory.closed_timemap sc0 mem0)
+    :
+      exists cap1,
+        (<<STEPS: Trace.steps tr (Thread.mk _ st0 lc0 sc0 cap0) (Thread.mk _ st1 lc1 sc1 cap1)>>) /\
+        (<<SOUND: Memory.le mem1 cap1>>) /\
+        (<<SPACES:
+           forall loc ts (COV: covered loc ts cap1),
+             <<COV: covered loc ts mem1>> \/ spaces loc ts>>) /\
+        (<<LEFTS:
+           forall loc ts (UNATACHABLE: unattachable cap1 loc ts),
+             <<COV: unattachable mem1 loc ts>> \/ lefts loc ts>>).
+  Proof.
+    remember (Thread.mk lang st0 lc0 sc0 mem0).
+    remember (Thread.mk lang st1 lc1 sc1 mem1). ginduction STEPS.
+    { i. clarify. esplits; eauto. }
+    { i. clarify. inv EVENTS. ss. des.
+      exploit Thread.step_future; eauto. i. des.
+      destruct th1. ss. exploit step_lifting; eauto. i. des.
+      exploit IHSTEPS; eauto. i. des. exists cap2. splits; auto. econs; eauto.
+    }
+  Qed.
+
+End LIFT.
+
+
+Fixpoint intervals_sum (l: list (Loc.t * Interval.t)):
+  Loc.t -> Time.t -> Prop :=
+  match l with
+  | [] => bot2
+  | (loc, (from, to))::tl =>
+    fun loc0 ts0 =>
+      (loc0 = loc /\ Interval.mem (from, to) ts0) \/
+      intervals_sum tl loc0 ts0
+  end.
+
+Fixpoint intervals_sum_left (l: list (Loc.t * Interval.t)):
+  Loc.t -> Time.t -> Prop :=
+  match l with
+  | [] => bot2
+  | (loc, (from, to))::tl =>
+    fun loc0 ts0 =>
+      (loc0 = loc /\ Time.le from ts0 /\ Time.lt ts0 to) \/
+      intervals_sum_left tl loc0 ts0
+  end.
+
+Lemma intervals_sum_interval l
+      loc ts
+  :
+    intervals_sum l loc ts <->
+    exists from to,
+      (<<IN: List.In (loc, (from, to)) l>>) /\ (<<ITV: Interval.mem (from, to) ts>>).
+Proof.
+  ginduction l; ss.
+  { i; split; i; ss. des. ss. }
+  { i; split; i; ss.
+    { destruct a. destruct t0. des; clarify.
+      { esplits; eauto. }
+      { eapply IHl in H. des. esplits; eauto. }
+    }
+    { destruct a. destruct t0. des; clarify; eauto. right.
+      eapply IHl. eauto. }
+  }
+Qed.
+
+Lemma intervals_sum_left_interval l
+      loc ts
+  :
+    intervals_sum_left l loc ts <->
+    exists from to,
+      (<<IN: List.In (loc, (from, to)) l>>) /\ (<<FROM: Time.le from ts>>) /\ (<<TO: Time.lt ts to>>).
+Proof.
+  ginduction l; ss.
+  { i; split; i; ss. des. ss. }
+  { i; split; i; ss.
+    { destruct a. destruct t0. des; clarify.
+      { esplits; eauto. }
+      { eapply IHl in H. des. esplits; eauto. }
+    }
+    { destruct a. destruct t0. des; clarify; eauto. right.
+      eapply IHl. eauto. }
+  }
+Qed.
+
+
+Definition is_reserving (te: ThreadEvent.t): Prop :=
+  match te with
+  | ThreadEvent.promise _ _ _ Message.reserve Memory.op_kind_add => True
+  | _ => False
+  end.
+
+Lemma promise_needed_spaces prom0 prom1 mem0 mem1
+      loc from to msg kind
+      (PROMISE: Memory.promise prom0 mem0 loc from to msg prom1 mem1 kind)
+      (WF: kind <> Memory.op_kind_cancel)
+  :
+    ((<<ALREADY: forall ts (ITV: Interval.mem (from, to) ts), covered loc ts mem0>>) /\
+     (<<COVERED: forall loc ts, covered loc ts mem1 <-> covered loc ts mem0>>))
+    \/
+    ((<<NEW: forall ts (ITV: Interval.mem (from, to) ts), ~ covered loc ts mem0>>) /\
+     (<<COVERED: forall loc0 ts0,
+         covered loc0 ts0 mem1 <-> covered loc0 ts0 mem0 \/ (loc0 = loc /\ Interval.mem (from, to) ts0)>>) /\
+     (<<WF: Time.lt from to>>))
+.
+Proof.
+  inv PROMISE.
+  { right. exploit add_succeed_wf; try apply MEM. i. des. splits; auto.
+    { ii. inv H. eapply DISJOINT; eauto. }
+    { i. erewrite (@add_covered mem1); eauto. }
+  }
+  { left. exploit split_succeed_wf; try apply MEM. i. des. splits; auto.
+    { ii. econs; eauto. eapply Interval.le_mem; eauto. econs; ss.
+      { refl. }
+      { left. auto. }
+    }
+    { i. eapply split_covered; eauto. }
+  }
+  { left. exploit lower_succeed_wf; try apply MEM. i. des. splits; auto.
+    { ii. econs; eauto. }
+    { i. eapply lower_covered; eauto. }
+  }
+  { ss. }
+Qed.
+
+Lemma step_needed_spaces lang (th0 th1: Thread.t lang) pf e
+      (times: Loc.t -> Time.t -> Prop)
+      (STEP: Thread.step pf e th0 th1)
+      (NOTCANCEL: ~ is_cancel e)
+      (WFTIME: wf_time_evt times e)
+  :
+    ((<<ALREADY: write_not_in (fun loc0 ts0 => ~ covered loc0 ts0 th0.(Thread.memory)) e>>) /\
+     (<<COVERED: forall loc ts, covered loc ts th1.(Thread.memory) <-> covered loc ts th0.(Thread.memory)>>))
+    \/
+    exists loc from to,
+      (<<NEW: forall ts (ITV: Interval.mem (from, to) ts), ~ covered loc ts th0.(Thread.memory)>>) /\
+      (<<COVERED: forall loc0 ts0,
+          covered loc0 ts0 th1.(Thread.memory) <-> covered loc0 ts0 th0.(Thread.memory) \/ (loc0 = loc /\ Interval.mem (from, to) ts0)>>) /\
+      (<<WF: Time.lt from to>>) /\
+      (<<TIMES: times loc from /\ times loc to>>) /\
+      (<<EVENT: write_not_in (fun loc0 ts0 => ~ (loc0 = loc /\ Interval.mem (from, to) ts0)) e>>).
+Proof.
+  inv STEP.
+  { inv STEP0. inv LOCAL. ss.
+    destruct (Memory.op_kind_is_cancel kind) eqn:KIND.
+    { destruct kind; ss. }
+    exploit promise_needed_spaces; eauto.
+    { destruct kind; ss. }
+    i. des.
+    { left. splits; auto. }
+    { right. esplits; eauto. }
+  }
+  { inv STEP0. inv LOCAL; try by (splits; eauto); ss.
+    { ss. inv LOCAL0. inv WRITE.
+      exploit promise_needed_spaces; eauto.
+      { destruct kind; ss. inv PROMISE; ss. }
+      i. des.
+      { left. esplits; eauto. }
+      { right. esplits; eauto. }
+    }
+    { ss. inv LOCAL2. inv WRITE.
+      exploit promise_needed_spaces; eauto.
+      { destruct kind; ss. inv PROMISE; ss. }
+      i. des.
+      { left. esplits; eauto. }
+      { right. esplits; eauto. }
+    }
+  }
+Qed.
+
+
+Inductive reservations_added:
+  forall (l: list (Loc.t * Interval.t)) (mem0 mem1: Memory.t), Prop :=
+| reservations_added_base
+    mem0
+  :
+    reservations_added [] mem0 mem0
+| reservations_added_cons
+    mem0 mem1 mem2 loc from to tl
+    (ADD: Memory.add mem0 loc from to Message.reserve mem1)
+    (TL: reservations_added tl mem1 mem2)
+    (WF: Time.lt from to)
+  :
+    reservations_added ((loc, (from, to))::tl) mem0 mem2
+.
+
+Lemma reservations_added_trans l0 l1 mem0 mem1 mem2
+      (ADDED0: reservations_added l0 mem0 mem1)
+      (ADDED1: reservations_added l1 mem1 mem2)
+  :
+    reservations_added (l0 ++ l1) mem0 mem2.
+Proof.
+  ginduction l0; eauto.
+  { i. inv ADDED0. ss. }
+  { i. inv ADDED0. exploit IHl0; eauto. i. econs; eauto. }
+Qed.
+
+
+Lemma reservations_added_cancel
+      loc from to mem0 mem1 mem2 tl
+      (CANCEL: Memory.remove mem1 loc from to Message.reserve mem0)
+      (TL: reservations_added tl mem1 mem2)
+      (WF: Time.lt from to)
+  :
+    reservations_added ((loc, (from, to))::tl) mem0 mem2.
+Proof.
+  econs; eauto.
+  exploit (@Memory.add_exists mem0 loc from to Message.reserve); eauto.
+  { i. erewrite Memory.remove_o in GET2; eauto. des_ifs.
+    exploit Memory.get_disjoint.
+    { eapply GET2. }
+    { eapply Memory.remove_get0; eauto. }
+    i. ss. des; clarify. symmetry. auto.
+  }
+  { econs. }
+  i. des. replace mem1 with mem3; auto. eapply Memory.ext.
+  i. erewrite (@Memory.add_o mem3 mem0); eauto.
+  erewrite (@Memory.remove_o mem0 mem1); eauto. des_ifs.
+  ss. des; clarify. symmetry. eapply Memory.remove_get0; eauto.
+Qed.
+
+Inductive disjoint_intervals
+  :
+    forall (l: list (Loc.t * Interval.t)), Prop :=
+| disjoint_base
+  :
+    disjoint_intervals []
+| disjoint_intervals_cons
+    loc from to tl
+    (TL: disjoint_intervals tl)
+    (NITV: forall ts (ITV: Interval.mem (from, to) ts),
+        ~ intervals_sum tl loc ts)
+    (TS: Time.lt from to)
+  :
+    disjoint_intervals ((loc, (from, to)) :: tl)
+.
+Hint Constructors disjoint_intervals.
+
+
+
+
+Lemma traced_steps_needed_spaces lang (th0 th1: Thread.t lang) tr
+      (times: Loc.t -> Time.t -> Prop)
+      (STEP: Trace.steps tr th0 th1)
+      (EVENTS: List.Forall (fun em => <<SAT: ((fun e => ~ is_cancel e) /1\ wf_time_evt times) (snd em)>>) tr)
+  :
+    exists l,
+      (<<WRITENOTIN:
+         List.Forall (fun em => <<SAT: write_not_in (fun loc ts => ~ (covered loc ts th0.(Thread.memory) \/ intervals_sum l loc ts)) (snd em)>>) tr>>) /\
+      (<<DISJOINT: disjoint_intervals l>>) /\
+      (<<NITV: forall loc ts (ITV: intervals_sum l loc ts), ~ covered loc ts th0.(Thread.memory)>>) /\
+      (<<COVERED: forall loc ts,
+          covered loc ts th1.(Thread.memory) <-> covered loc ts th0.(Thread.memory) \/ intervals_sum l loc ts>>) /\
+      (<<TIMES: List.Forall (fun locitv =>
+                               times (fst locitv) (fst (snd locitv)) /\
+                               times (fst locitv) (snd (snd locitv))) l>>)
+.
+Proof.
+  ginduction STEP; i.
+  { exists []. splits; auto. i. ss. split; auto. i. des; ss. }
+  { subst. inv EVENTS. des. exploit IHSTEP; eauto. i. des.
+    exploit step_needed_spaces; eauto. i. des.
+    { exists l. splits; auto.
+      { econs; eauto.
+        { eapply write_not_in_mon; eauto. i. ss.
+          eapply not_or_and in PR. des. auto. }
+        { eapply List.Forall_impl; eauto. i. ss.
+          eapply write_not_in_mon; eauto. i. ss.
+          erewrite COVERED0; eauto. }
+      }
+      { i. erewrite <- COVERED0; eauto. }
+      { i. erewrite <- COVERED0. eauto. }
+    }
+    { exists ((loc, (from, to)) :: l). splits.
+      { econs.
+        { eapply write_not_in_mon; eauto. ss. i.
+          ii. des. eapply PR. eauto. }
+        { eapply List.Forall_impl; try apply WRITENOTIN; eauto. i. ss.
+          eapply write_not_in_mon; eauto. i. ss.
+          ii. eapply PR. des; auto. eapply COVERED0 in H3. des; auto. }
+      }
+      { econs; eauto. ii. eapply NITV; eauto. eapply COVERED0. auto. }
+      { i. ss. des; clarify; eauto.
+        eapply NITV in ITV. ii. eapply ITV. eapply COVERED0. auto. }
+      { ii. erewrite COVERED. erewrite COVERED0. ss. split; i; des; auto. }
+      { econs; ss. }
+    }
+  }
+Qed.
+
+Lemma reserve_empty_intervals times lang (th: Thread.t lang) l
+      (DISJOINT: disjoint_intervals l)
+      (NITV: forall loc ts (ITV: intervals_sum l loc ts),
+          ~ covered loc ts th.(Thread.memory))
+      (MLE: Memory.le th.(Thread.local).(Local.promises) th.(Thread.memory))
+      (TIMES: List.Forall (fun locitv =>
+                             times (fst locitv) (fst (snd locitv)) /\
+                             times (fst locitv) (snd (snd locitv))) l)
+  :
+    exists tr prom' mem',
+      (<<STEPS: Trace.steps tr th (Thread.mk _ th.(Thread.state) (Local.mk th.(Thread.local).(Local.tview) prom') th.(Thread.sc) mem')>>) /\
+      (<<RESERVETRACE: List.Forall (fun em => <<SAT: (is_reserving /1\ wf_time_evt times) (snd em)>>) tr>>) /\
+      (<<ADDEDPROM: reservations_added l th.(Thread.local).(Local.promises) prom'>>) /\
+      (<<ADDEDMEM: reservations_added l th.(Thread.memory) mem'>>)
+.
+Proof.
+  ginduction l; i.
+  { destruct th. destruct local. ss. exists []. esplits; eauto.
+    { econs. }
+    { econs. }
+  }
+  { inv DISJOINT. inv TIMES. ss.
+    exploit (@Memory.add_exists th.(Thread.memory) loc from to Message.reserve); eauto.
+    { ii. eapply NITV.
+      { left. eauto. }
+      { econs; eauto. }
+    }
+    { econs. }
+    intros [mem MEM].
+    exploit (@Memory.add_exists_le th.(Thread.local).(Local.promises) th.(Thread.memory)); eauto.
+    intros [prom PROM].
+    assert (STEP: Thread.step false (ThreadEvent.promise loc from to Message.reserve Memory.op_kind_add) th (Thread.mk _ th.(Thread.state) (Local.mk th.(Thread.local).(Local.tview) prom) th.(Thread.sc) mem)).
+    { destruct th. ss. econs. econs; ss. econs; ss. econs; ss. }
+    exploit (@IHl times lang (Thread.mk _ th.(Thread.state) (Local.mk th.(Thread.local).(Local.tview) prom) th.(Thread.sc) mem)); eauto; ss.
+    { i. erewrite add_covered; eauto. ii. des; subst.
+      { eapply NITV; eauto. }
+      { eapply NITV0; eauto. }
+    }
+    { hexploit step_promises_le; eauto.
+      { econs; eauto. }
+      i. ss.
+    }
+    i. des. esplits.
+    { econs; eauto. }
+    { econs; ss. }
+    { econs; eauto. }
+    { econs; eauto. }
+  }
+Qed.
+
+Lemma reservations_added_get_same mem1 mem0 l
+      (ADDED: reservations_added l mem0 mem1)
+      loc ts
+      (NIN: forall from, ~ List.In (loc, (from, ts)) l)
+  :
+    Memory.get loc ts mem1 = Memory.get loc ts mem0.
+Proof.
+  ginduction ADDED; auto. i.
+  erewrite IHADDED; eauto.
+  { erewrite (@Memory.add_o mem1 mem0); eauto. des_ifs. ss. des; clarify.
+    exfalso. eapply NIN; eauto. }
+  { ii. ss. eapply NIN; eauto. }
+Qed.
+
+Lemma reservations_added_get_none mem1 mem0 l
+      (ADDED: reservations_added l mem0 mem1)
+      loc from ts
+      (IN: List.In (loc, (from, ts)) l)
+  :
+    Memory.get loc ts mem0 = None.
+Proof.
+  ginduction ADDED; ss. i. des; clarify.
+  { eapply Memory.add_get0; eauto. }
+  { eapply IHADDED in IN. erewrite Memory.add_o in IN; eauto. des_ifs. }
+Qed.
+
+Lemma reservations_added_le_le l mem0 mem1 cap1 cap0
+      (ADDED0: reservations_added l mem0 mem1)
+      (MLE: Memory.le mem1 cap1)
+      (ADDED1: reservations_added l cap0 cap1)
+  :
+    Memory.le mem0 cap0.
+Proof.
+  ii. destruct (classic (forall from, ~ List.In (loc, (from, to)) l)).
+  { erewrite <- (@reservations_added_get_same cap1 cap0); eauto.
+    erewrite <- (@reservations_added_get_same mem1 mem0) in LHS; eauto. }
+  { eapply not_all_not_ex in H. des.
+    erewrite reservations_added_get_none in LHS; eauto. ss. }
+Qed.
+
+Lemma cancel_reservations_added times l prom lang lc
+      (ADDEDPROM: reservations_added l prom lc.(Local.promises))
+      (TIMES: List.Forall (fun locitv =>
+                             times (fst locitv) (fst (snd locitv)) /\
+                             times (fst locitv) (snd (snd locitv))) l)
+  :
+    exists tr,
+      (<<CANCELTRACE: List.Forall (fun em => <<SAT: (is_cancel /1\ wf_time_evt times) (snd em)>>) tr>>) /\
+    forall
+      (st: Language.state lang) sc mem
+      (MLE: Memory.le lc.(Local.promises) mem),
+    exists mem',
+      (<<STEPS: Trace.steps tr (Thread.mk _ st lc sc mem) (Thread.mk _ st (Local.mk lc.(Local.tview) prom) sc mem')>>) /\
+      (<<ADDEDMEM: reservations_added l mem' mem>>)
+.
+Proof.
+  ginduction l; i.
+  { exists []. splits; ss. i. destruct lc. ss. inv ADDEDPROM. esplits; eauto. econs. }
+  { inv TIMES. inv ADDEDPROM.
+    exploit IHl; eauto. i. des.
+    eexists (tr++[(Local.mk lc.(Local.tview) mem1, ThreadEvent.promise loc from to Message.reserve Memory.op_kind_cancel)]).
+    splits.
+    { eapply Forall_app; eauto. econs; ss. }
+    i. exploit (x0 st sc mem); eauto. i. des.
+    exploit (@Memory.remove_exists mem1 loc from to Message.reserve); eauto.
+    { eapply Memory.add_get0; eauto. } i. des.
+    exploit (@Memory.remove_exists_le mem1 mem'); eauto.
+    { eapply trace_steps_promises_le in STEPS; eauto. } i. des.
+    assert (mem2 = prom).
+    { symmetry. eapply MemoryMerge.add_remove; eauto. } subst.
+    esplits.
+    { eapply Trace.steps_trans.
+      { eapply STEPS. }
+      { econs; eauto. econs 1; eauto. econs; eauto. }
+    }
+    { eapply reservations_added_cancel; eauto. }
+  }
+Qed.
+
+Lemma step_finte_write_to (e: ThreadEvent.t)
+      (times: Loc.t -> Time.t -> Prop)
+      (EVENT: wf_time_evt times e)
+  :
+    exists (l: list (Loc.t * Time.t)),
+      (<<EVENT: write_not_to (fun loc ts => ~ List.In (loc, ts) l) e>>) /\
+      (<<TIMES: List.Forall (fun locts => times (fst locts) (snd locts)) l>>).
+Proof.
+  destruct e; try by (exists []; esplits; eauto); ss.
+  { exists [(loc, to)]. esplits; ss.
+    { des_ifs. ii. eapply H. auto. }
+    { econs; ss. des. auto. }
+  }
+  { exists [(loc, to)]. esplits; ss.
+    { ii. eapply H. auto. }
+    { econs; ss. des. auto. }
+  }
+  { exists [(loc, tsw)]. esplits; ss.
+    { ii. eapply H. auto. }
+    { econs; ss. des. auto. }
+  }
+Qed.
+
+Lemma write_not_to_mon P0 P1
+      (LE: P0 <2= P1)
+  :
+    write_not_to P1 <1= write_not_to P0.
+Proof.
+  ii. unfold write_not_to in *. des_ifs; auto.
+Qed.
+
+Lemma traced_steps_finte_write_to (tr: Trace.t)
+      (times: Loc.t -> Time.t -> Prop)
+      (EVENTS: List.Forall (fun em => <<SAT: (wf_time_evt times) (snd em)>>) tr)
+  :
+    exists (l: list (Loc.t * Time.t)),
+      (<<EVENTS: List.Forall (fun em => write_not_to (fun loc ts => ~ List.In (loc, ts) l) (snd em)) tr>>) /\
+      (<<TIMES: List.Forall (fun locts => times (fst locts) (snd locts)) l>>).
+Proof.
+  ginduction tr.
+  { i. inv EVENTS. exists []. esplits; eauto. }
+  { i. inv EVENTS. exploit IHtr; eauto. i. des.
+    exploit (@step_finte_write_to (snd a)); eauto. i. des.
+    exists (l0 ++ l). esplits; eauto.
+    { econs; eauto.
+      { eapply write_not_to_mon; eauto. ii. eapply PR. eapply List.in_or_app; eauto. }
+      { eapply List.Forall_impl; eauto. i. ss.
+        eapply write_not_to_mon; eauto. ii. eapply PR. eapply List.in_or_app; eauto. }
+    }
+    { eapply Forall_app; eauto. }
+  }
+Qed.
+
+Lemma reserve_write_to (times: Loc.t -> Time.t -> Prop)
+      (DIVERGE: forall loc ts,
+          exists ts',
+            (<<TIMES: times loc ts'>>) /\
+            (<<TS: Time.lt ts ts'>>))
+      mem
+      (MWF: memory_times_wf times mem)
+      loc ts
+      (TIMES: times loc ts)
+  :
+    (<<ALREADY: unattachable mem loc ts>>) \/
+    (<<NEW: exists from mem',
+        (<<TS: Time.lt ts from>>) /\
+        (<<ADD: Memory.add mem loc ts from Message.reserve mem'>>) /\
+        (<<TIMES: times loc from>>) /\
+        (<<MWF: memory_times_wf times mem'>>)>>).
+Proof.
+  destruct (classic (unattachable mem loc ts)); auto. right.
+  hexploit (@cell_elements_least
+              (mem loc)
+              (fun to => exists from msg,
+                   (<<GET: Memory.get loc to mem = Some (from, msg)>>) /\
+                   (<<TS: Time.lt ts from>>))).
+  i. des.
+  { hexploit (@Memory.add_exists mem loc ts from0 Message.reserve); ss.
+    { ii. destruct (Time.le_lt_dec from2 ts).
+      { eapply H. econs; eauto.
+        inv LHS. inv RHS. ss. eapply TimeFacts.lt_le_lt; eauto. }
+      { dup GET2. eapply LEAST in GET2.
+        { exploit memory_get_to_mon.
+          { eapply GET1. }
+          { eapply GET0. }
+          { inv LHS. inv RHS. ss. eapply TimeFacts.lt_le_lt; eauto. }
+          i. timetac.
+        }
+        esplits; eauto.
+      }
+    }
+    { econs. }
+    i. des. esplits; eauto.
+    { eapply MWF in GET0. des; auto. }
+    { eapply MWF in GET0. des.
+      ii. erewrite Memory.add_o in GET0; eauto. des_ifs.
+      { ss. des; clarify. }
+      { eapply MWF; eauto. }
+    }
+  }
+  { hexploit (DIVERGE loc ts). i. des.
+    hexploit (@Memory.add_exists mem loc ts ts' Message.reserve); ss.
+    { ii. eapply EMPTY; eauto. esplits; eauto.
+      destruct (Time.le_lt_dec from2 ts); auto. exfalso.
+      eapply H. econs; eauto.
+      inv LHS. inv RHS. ss. eapply TimeFacts.lt_le_lt; eauto. }
+    { econs. }
+    i. des. esplits; eauto.
+    ii. erewrite Memory.add_o in GET; eauto. des_ifs.
+    { ss. des; clarify. }
+    { eapply MWF; eauto. }
+  }
+Qed.
+
+Lemma reserve_write_tos times lang (th: Thread.t lang) tos
+      (DIVERGE: forall loc ts,
+          exists ts',
+            (<<TIMES: times loc ts'>>) /\
+            (<<TS: Time.lt ts ts'>>))
+      (MWF: memory_times_wf times th.(Thread.memory))
+      (MLE: Memory.le th.(Thread.local).(Local.promises) th.(Thread.memory))
+      (TIMES: List.Forall (fun locts => times (fst locts) (snd locts)) tos)
+  :
+    exists l tr prom' mem',
+      (<<STEPS: Trace.steps tr th (Thread.mk _ th.(Thread.state) (Local.mk th.(Thread.local).(Local.tview) prom') th.(Thread.sc) mem')>>) /\
+      (<<RESERVETRACE: List.Forall (fun em => <<SAT: (is_reserving /1\ wf_time_evt times) (snd em)>>) tr>>) /\
+      (<<ADDEDPROM: reservations_added l th.(Thread.local).(Local.promises) prom'>>) /\
+      (<<ADDEDMEM: reservations_added l th.(Thread.memory) mem'>>) /\
+      (<<WRITETO: forall loc ts (IN: List.In (loc, ts) tos),
+          unattachable mem' loc ts>>) /\
+      (<<TIMES: List.Forall (fun locitv =>
+                               times (fst locitv) (fst (snd locitv)) /\
+                               times (fst locitv) (snd (snd locitv))) l>>)
+.
+Proof.
+  ginduction tos; i; ss.
+  { exists [], []. destruct th. destruct local. ss. esplits; eauto; ss.
+    { econs. }
+    { econs. }
+  }
+  { inv TIMES. exploit IHtos; eauto. i. des.
+    exploit reserve_write_to.
+    { eauto. }
+    { eapply memory_times_wf_traced in STEPS; eauto.
+      eapply List.Forall_impl; eauto. i. ss. des; auto. }
+    { eauto. }
+    i. ss. des.
+    { exists l, tr. esplits; eauto. i. des; auto. clarify. }
+    { exploit (@Memory.add_exists_le prom' mem'); eauto.
+      { eapply trace_steps_promises_le in STEPS; eauto. }
+      i. des.
+      assert (PROM: Memory.promise prom' mem' (fst a) (snd a) from Message.reserve promises2 mem'0 Memory.op_kind_add).
+      { econs; eauto. ss. }
+      destruct th. esplits.
+      { eapply Trace.steps_trans.
+        { eauto. }
+        { econs 2.
+          { econs 1. econs; eauto. }
+          { econs 1. }
+          { ss. }
+        }
+      }
+      { eapply Forall_app; eauto. econs; ss. }
+      { ss. eapply reservations_added_trans.
+        { eauto. }
+        { econs; eauto. econs. }
+      }
+      { ss. eapply reservations_added_trans.
+        { eauto. }
+        { econs; eauto. econs. }
+      }
+      { i. erewrite add_unattachable; eauto. des; clarify.
+        { right. splits; ss. refl. }
+        { eauto. }
+      }
+      { eapply Forall_app; eauto. }
+    }
+  }
+Qed.
+
+
+
+Lemma reservations_added_non_covered l mem0 mem1
+      (ADDED: reservations_added l mem0 mem1)
+      loc ts
+      (COVERED: covered loc ts mem0)
+  :
+    ~ intervals_sum l loc ts.
+Proof.
+  ginduction l; eauto. i. inv ADDED. ss. ii.
+  des; clarify.
+  { inv COVERED. eapply add_succeed_wf in ADD. des.
+    eapply DISJOINT; eauto. }
+  { eapply IHl; eauto. erewrite add_covered; eauto. }
+Qed.
+
+Lemma add_unattachable_disjoint mem1 mem0 loc from to msg
+      (ADD: Memory.add mem0 loc from to msg mem1)
+      loc0 ts0
+      (UNATTACHABLE: unattachable mem0 loc0 ts0)
+  :
+    ~ (loc0 = loc /\ Time.le from ts0 /\ Time.lt ts0 to).
+Proof.
+  ii. des; subst. inv UNATTACHABLE.
+  exploit add_succeed_wf; eauto. i. des.
+  hexploit DISJOINT; eauto. i. eapply disjoint_equivalent2 in H. des; ss.
+  { eapply TS1. eapply TimeFacts.le_lt_lt; eauto. }
+  { eapply Time.lt_strorder. eapply TimeFacts.le_lt_lt.
+    { eapply TS0. } eapply TimeFacts.le_lt_lt.
+    { instantiate (1:=ts0). unfold Time.join. des_ifs. }
+    { unfold Time.meet. des_ifs. }
+  }
+Qed.
+
+Lemma reservations_added_non_unattachable l mem0 mem1
+      (ADDED: reservations_added l mem0 mem1)
+      loc ts
+      (UNATTACHABLE: unattachable mem0 loc ts)
+  :
+    ~ intervals_sum_left l loc ts.
+Proof.
+  ginduction l; eauto. i. inv ADDED. ss. ii.
+  des; clarify.
+  { exploit add_unattachable_disjoint; eauto. }
+  { eapply IHl; eauto. erewrite add_unattachable; eauto. }
+Qed.
+
+Lemma reservations_added_unattachable l mem0 mem1
+      (ADDED: reservations_added l mem0 mem1)
+      loc ts
+      (UNATTACHABLE: unattachable mem1 loc ts)
+  :
+    unattachable mem0 loc ts \/ intervals_sum_left l loc ts.
+Proof.
+  ginduction l; eauto. i.
+  { inv ADDED. auto. }
+  { i. inv ADDED. eapply IHl in TL; eauto. ss.
+    erewrite add_unattachable in TL; eauto. des; auto. }
+Qed.
+
+Lemma can_reserve_all_needed times
+      (DIVERGE: forall loc ts,
+          exists ts',
+            (<<TIMES: times loc ts'>>) /\
+            (<<TS: Time.lt ts ts'>>))
+      lang
+      st0 st1 lc0 lc1 sc0 sc1 mem0 mem1 tr
+      (MWF: memory_times_wf times mem0)
+      (STEPS: Trace.steps tr (Thread.mk lang st0 lc0 sc0 mem0) (Thread.mk lang st1 lc1 sc1 mem1))
+      (EVENTS: List.Forall (fun em => <<SAT: ((fun e => ~ is_cancel e) /1\ wf_time_evt times) (snd em)>>) tr)
+      (MEM: Memory.closed mem0)
+      (LOCAL: Local.wf lc0 mem0)
+      (SC: Memory.closed_timemap sc0 mem0)
+  :
+    exists lc0' mem0' tr_reserve tr_cancel,
+      (<<RESERVESTEPS:
+         Trace.steps tr_reserve (Thread.mk lang st0 lc0 sc0 mem0) (Thread.mk lang st0 lc0' sc0 mem0')>>) /\
+      (<<RESERVETRACE:
+         List.Forall (fun em => <<SAT: (is_reserving /1\ wf_time_evt times) (snd em)>>) tr_reserve>>) /\
+      (<<CANCELTRACE: List.Forall (fun em => <<SAT: (is_cancel /1\ wf_time_evt times) (snd em)>>) tr_cancel>>) /\
+      (<<CAP:
+         forall cap0'
+                (MLE: Memory.le mem0' cap0'),
+         exists cap0 cap1 ,
+           (<<CANCELSTEPS:
+              Trace.steps tr_cancel (Thread.mk lang st0 lc0' sc0 cap0') (Thread.mk lang st0 lc0 sc0 cap0)>>) /\
+           (<<STEPS:
+              Trace.steps tr (Thread.mk lang st0 lc0 sc0 cap0) (Thread.mk lang st1 lc1 sc1 cap1)>>)>>).
+Proof.
+  exploit (@traced_steps_finte_write_to tr); eauto.
+  { eapply List.Forall_impl; eauto. i. ss. des. eauto. }
+  intros [tos ?]. des.
+  exploit traced_steps_needed_spaces; eauto.
+  i. des.
+  exploit reserve_empty_intervals; eauto.
+  { eapply LOCAL. }
+  i. des. ss.
+  assert (MLE: Memory.le prom' mem').
+  { eapply trace_steps_promises_le in STEPS0; eauto. eapply LOCAL. }
+  exploit reserve_write_tos.
+  { eauto. }
+  { eapply memory_times_wf_traced in STEPS0; eauto.
+    eapply List.Forall_impl; eauto. i. ss. des. eauto.
+  }
+  { ss. }
+  { eauto. }
+  i. des. ss.
+  assert (ADDEDPROMALL: reservations_added (l ++ l0) (Local.promises lc0) prom'0).
+  { eapply reservations_added_trans; eauto. }
+  assert (ADDEDMEMALL: reservations_added (l ++ l0) mem0 mem'0).
+  { eapply reservations_added_trans; eauto. }
+  hexploit cancel_reservations_added.
+  { instantiate (1:=Local.mk lc0.(Local.tview) prom'0). eapply ADDEDPROMALL. }
+  { eapply Forall_app; eauto. }
+  i. des.
+  esplits.
+  { eapply Trace.steps_trans.
+    { eapply STEPS0. }
+    { eapply STEPS1. }
+  }
+  { eapply Forall_app; eauto. }
+  { eapply CANCELTRACE. }
+  { i. ss. exploit (H0 st0 sc0 cap0').
+    { etrans; eauto. eapply trace_steps_promises_le in STEPS1; eauto. }
+    i. des.
+    assert (MLE1: Memory.le mem0 mem'1).
+    { eapply reservations_added_le_le.
+      { eapply ADDEDMEMALL. }
+      { eapply MLE0. }
+      { eauto. }
+    }
+    hexploit traced_step_lifting.
+    { eapply STEPS. }
+    { eapply list_Forall_sum.
+      { eapply list_Forall_sum.
+        { eapply EVENTS. }
+        { eapply EVENTS0. }
+        { instantiate (1:=fun em => <<SAT: ((fun e => ~ is_cancel e) /1\ write_not_to (fun loc ts => ~ List.In (loc, ts) tos)) (snd em)>>).
+          i. ss. des. splits; auto. }
+      }
+      { eapply WRITENOTIN. }
+      i. ss. des. splits; eauto.
+    }
+    { eapply MLE1. }
+    { i. destruct (classic (covered loc ts mem0)); auto. right.
+      ii. des; ss. eapply reservations_added_non_covered in ADDEDMEM1; eauto.
+      eapply ADDEDMEM1. erewrite intervals_sum_interval.
+      erewrite intervals_sum_interval in H1. des. esplits; eauto.
+      eapply List.in_or_app; eauto. }
+    { i. destruct (classic (unattachable mem0 loc ts)); auto. right.
+      ii. des; ss. eapply reservations_added_non_unattachable in ADDEDMEM1; eauto.
+      eapply ADDEDMEM1. erewrite intervals_sum_left_interval.
+      eapply WRITETO in H1. eapply reservations_added_unattachable in H1; eauto.
+      des; ss. }
+    { eauto. }
+    { eauto. }
+    { eauto. }
+    i. des. exists mem'1, cap1.
+    splits; eauto. destruct lc0. ss.
+  }
+Qed.
